Cleanup, factored out similar proofs.

easycrypt/KEM.ec
@@ -8,226 +8,198 @@
  * ROM for the underlying agile KEF.
  *
  *)
+
 require import Bool.
 require import Int.
 require import Real.
-require import FMap.
 require import Pair.
+require import FMap.
+
 import FSet.
 import OptionGet.
 
 lemma eq_except_in_dom : 
   forall (m1 m2:('a, 'b) map) (x y:'a),
-   eq_except m1 m2 x => x <> y => (in_dom y m1 <=> in_dom y m2) 
+    eq_except m1 m2 x => x <> y => (in_dom y m1 <=> in_dom y m2) 
 by [].
 
 lemma eq_except_set :
   forall (m1 m2:('a, 'b) map) (x y:'a) (z:'b),
-   eq_except m1 m2 x => eq_except m1.[y <- z] m2.[y <- z] x 
+    eq_except m1 m2 x => eq_except m1.[y <- z] m2.[y <- z] x 
 by [].
 
+
+(* TODO: Map this to a RO in the standard library *)
 theory Agile_KEF.
 
- type parameter.
- type secret.
- type key.
-
- op key : key distr.
- 
- axiom lossless_key : Distr.weight key = 1%r.
-
- module type KEF = {
-  fun init() : unit {*}
-  fun extract(p:parameter, s:secret) : key
- }.
-
- module type Oracles = {
-  fun extract(p:parameter, s:secret) : key
- }.
+  type parameter.
+  type secret.
+  type key.
+  
+  module type KEF = {
+    fun init() : unit {*}
+    fun extract(p:parameter, s:secret) : key
+  }.
+  
+  module type Oracle = {
+    fun extract(p:parameter, s:secret) : key
+  }.
 
 end Agile_KEF.
 
 
 theory Agile_Labeled_KEM.
-
- type parameter.
- type pkey.
- type skey.
- type key.
- type label.
- type ciphertext.
-
- op key : key distr.
-
- axiom lossless_key : Distr.weight key = 1%r.
-
- (* Decryption is functional *)
- op decrypt : parameter -> skey -> label -> ciphertext -> key.
-
- (* TODO: keep abstract *)
- pred keypair (pk:pkey, sk:skey) = true.
-
- module type KEM = {
-  fun init() : unit {*}
-  fun keygen() : pkey * skey
-  fun enc(p:parameter, pk:pkey, t:label) : key * ciphertext
-  fun dec(p:parameter, sk:skey, t:label, c:ciphertext) : key
- }.
-
- theory RCCA.
-
-  const P : parameter set.
-
-  const p' : parameter.
-
-  axiom p'_in_P : mem p' P.
-
-  module type Oracles = {
-   fun dec(p:parameter, t:label, c:ciphertext) : key option
-  }.
-
-  module type Adversary(O:Oracles) = {
-   fun choose(pk:pkey) : label
-   fun guess(c:ciphertext, k:key) : bool
-  }.
   
-  module RCCA(KEM:KEM, A:Adversary) = {
-   var pk : pkey
-   var sk : skey
-   var keys : key set
-   var labels : label set
+  type parameter.
+  type pkey.
+  type skey.
+  type key.
+  type label.
+  type ciphertext.
+    
+  module type KEM = {
+    fun init() : unit {*}
+    fun keygen() : pkey * skey
+    fun enc(p:parameter, pk:pkey, t:label) : key * ciphertext
+    fun dec(p:parameter, sk:skey, t:label, c:ciphertext) : key
+  }.
+
+  theory RCCA.
+  
+    const P : parameter set.
    
-   module O = {  
-    fun dec(p:parameter, t:label, c:ciphertext) : key option = {
-      var k : key;
-      var maybe_k : key option = None;
-      if (!mem t labels /\ mem p P) { 
-        labels = add t labels;
-        k = KEM.dec(p, sk, t, c);
-        maybe_k = if (!mem k keys) then Some k else None;
+    const pp : parameter.
+   
+    axiom pp_in_P : mem pp P.
+  
+    op key : key distr.
+     
+    module type Oracle = {
+      fun dec(p:parameter, t:label, c:ciphertext) : key option
+    }.
+   
+    module type Adversary(O:Oracle) = {
+      fun choose(pk:pkey) : label
+      fun guess(c:ciphertext, k:key) : bool
+    }.
+  
+    module W = {
+      var pk : pkey
+      var sk : skey
+      var keys : key set
+      var labels : label set
+    }.
+    
+    module Wrap(KEM:KEM) : Oracle = {  
+      fun dec(p:parameter, t:label, c:ciphertext) : key option = {
+        var k : key;
+        var maybe_k : key option = None;
+        if (!mem t W.labels /\ mem p P) { 
+          W.labels = add t W.labels;
+          k = KEM.dec(p, W.sk, t, c);
+          maybe_k = if (!mem k W.keys) then Some k else None;
+        }
+        return maybe_k;
       }
-      return maybe_k;
-    }
-   }
-   
-   module A = A(O)
+    }.
+    
+    module RCCA(KEM:KEM, A:Adversary) = {
+      module O = Wrap(KEM)
+      module A = A(O)
+     
+      fun main() : bool = {
+        var b, b', valid : bool;
+        var k0, k1 : key;
+        var c : ciphertext;
+        var t : label;
+        KEM.init();
+        (W.pk, W.sk) = KEM.keygen();
+        W.keys = FSet.empty;
+        W.labels = FSet.empty;
+        t = A.choose(W.pk);
+        valid = !mem t W.labels; 
+        (k0, c) = KEM.enc(pp, W.pk, t);
+        k1 = $key;
+        b = ${0,1};
+        W.keys = add k0 (add k1 W.keys);
+        b' = A.guess(c, if b then k1 else k0);
+        return (b = b' /\ valid);
+      }
+    }.
   
-   fun main() : bool = {
-     var b, b', valid : bool;
-     var k0, k1 : key;
-     var c : ciphertext;
-     var t : label;
-     KEM.init();
-     (pk, sk) = KEM.keygen();
-     keys = FSet.empty;
-     labels = FSet.empty;
-     t = A.choose(pk);
-     valid = !mem t labels; 
-     (k0, c) = KEM.enc(p', pk, t);
-     k1 = $key;
-     b = ${0,1};
-     keys = add k0 (add k1 keys);
-     b' = A.guess(c, if b then k1 else k0);
-     return (b = b' /\ valid);
-   }
-  }.
-
- end RCCA.
-
-
- theory OW_PCA.
-
-  const P : parameter set.
-
-  const p' : parameter.
-
-  axiom p'_in_P : mem p' P.
-
-  module type Oracles = {
-   fun check(p:parameter, k:key, t:label, c:ciphertext) : bool
-  }.
-
-  module type Adversary(O:Oracles) = {
-   fun choose(pk:pkey) : label
-   fun guess(c:ciphertext) : key 
-  }.
-
-  module OW_PCA(KEM:KEM, A:Adversary) = {
-   var sk : skey
-
-   module O = {
-    fun check(p:parameter, k:key, t:label, c:ciphertext) : bool = {
-      var k' : key;
-      k' = KEM.dec(p, sk, t, c);
-      return (k' = k);
-    }
-   }
+  end RCCA.
+  
+  
+  theory PCA.
+  
+    const P : parameter set.
    
-   module A = A(O)
-
-   fun main() : bool = {
-     var pk : pkey;
-     var t : label;
-     var k, k' : key;
-     var c : ciphertext;
-     KEM.init();
-     (pk, sk) = KEM.keygen();
-     t = A.choose(pk);
-     (k, c) = KEM.enc(p', pk, t);
-     k' = A.guess(c);
-     return (k = k');
-   }
-  }.
-
- end OW_PCA.
-
-
- theory NR_PCA.
-
-  const P : parameter set.
-
-  const p' : parameter.
-
-  axiom p'_in_P : mem p' P.
-
-  module type Oracles = {
-   fun check(p:parameter, k:key, t:label, c:ciphertext) : bool
-  }.
-
-  module type Adversary(O:Oracles) = {
-   fun choose(pk:pkey) : label
-   fun guess(c:ciphertext) : label * ciphertext
-  }.
-
-  module NR_PCA(KEM:KEM, A:Adversary) = {
-   var sk : skey
-
-   module O = {
-    fun check(p:parameter, k:key, t:label, c:ciphertext) : bool = {
-      var k' : key;
-      k' = KEM.dec(p, sk, t, c);
-      return (k' = k);
-    }
-   }
+    const pp : parameter.
    
-   module A = A(O)
+    axiom pp_in_P : mem pp P.
+   
+    module type Oracle = {
+      fun check(p:parameter, k:key, t:label, c:ciphertext) : bool
+    }.
 
-   fun main() : bool = {
-     var pk : pkey;
-     var t, t' : label;
-     var k, k' : key;
-     var c, c' : ciphertext;
-     KEM.init();
-     (pk, sk) = KEM.keygen();
-     t = A.choose(pk);
-     (k, c) = KEM.enc(p', pk, t);
-     (t', c') = A.guess(c);
-     k' = KEM.dec(p', sk, t', c');
-     return (c <> c' /\ k' = k);
-   }
-  }.
+    module type OW_Adversary(O:Oracle) = {
+      fun choose(pk:pkey) : label
+      fun guess(c:ciphertext) : key 
+    }.
 
- end NR_PCA.
+    module V = { var sk : skey }.
+    
+    module Wrap(KEM:KEM) : Oracle = {
+      fun check(p:parameter, k:key, t:label, c:ciphertext) : bool = {
+        var k' : key;
+        k' = KEM.dec(p, V.sk, t, c);
+        return (k' = k);
+      }
+    }.
+      
+    module OW_PCA(KEM:KEM, A:OW_Adversary) = {
+      module O = Wrap(KEM)
+      module A = A(O)
+    
+      fun main() : bool = {
+        var pk : pkey;
+        var t : label;
+        var k, k' : key;
+        var c : ciphertext;
+        KEM.init();
+        (pk, V.sk) = KEM.keygen();
+        t = A.choose(pk);
+        (k, c) = KEM.enc(pp, pk, t);
+        k' = A.guess(c);
+        return (k = k');
+      }
+    }.
+
+    module type NR_Adversary(O:Oracle) = {
+      fun choose(pk:pkey) : label
+      fun guess(c:ciphertext) : label * ciphertext
+    }.
+   
+    module NR_PCA(KEM:KEM, A:NR_Adversary) = {
+      module O = Wrap(KEM)
+      module A = A(O)
+    
+      fun main() : bool = {
+        var pk : pkey;
+        var t, t' : label;
+        var k, k' : key;
+        var c, c' : ciphertext;
+        KEM.init();
+        (pk, V.sk) = KEM.keygen();
+        t = A.choose(pk);
+        (k, c) = KEM.enc(pp, pk, t);
+        (t', c') = A.guess(c);
+        k' = KEM.dec(pp, V.sk, t', c');
+        return (c <> c' /\ k' = k);
+      }
+    }.
+  
+  end PCA.
 
 end Agile_Labeled_KEM.
 
@@ -238,1697 +210,1494 @@ type label.
 type pms.
 type ms.
 
+op key : ms distr.
+
+axiom key_lossless : Distr.weight key = 1%r.
+
 (* Shall we treat pv as a label or as a parameter? As a label for now *)
+(* Theory for non-agile pre-master secret KEM with protocol version as label *)
 clone import Agile_Labeled_KEM as Inner_KEM with 
- type parameter <- unit,
- type key <- pms,
- type label <- version.
+  type parameter <- unit,
+  type label     <- version,
+  type key       <- pms.
 
-clone Inner_KEM.OW_PCA as OW_PCA with op P = FSet.single ().
-
-clone Inner_KEM.NR_PCA as NR_PCA with op P = FSet.single ().
-
+(* Theory for agile and labeled master-secret KEM *)
 clone Agile_Labeled_KEM as Outer_KEM with 
- type pkey <- Inner_KEM.pkey,
- type skey <- Inner_KEM.skey,
- type key <- ms,
- type label <- label,
- type ciphertext <- Inner_KEM.ciphertext,
- type parameter <- version * hash.
+  type parameter  <- version * hash,
+  type label      <- label,
+  type key        <- ms,
+  type pkey       <- Inner_KEM.pkey,
+  type skey       <- Inner_KEM.skey,
+  type ciphertext <- Inner_KEM.ciphertext,
+  op RCCA.key     <- key.
 
-clone Outer_KEM.RCCA as RCCA.
+(* Theory for agile KEF, indexed by a hash algorithm identifier *)
+clone Agile_KEF as KEF with
+  type parameter <- hash,
+  type secret    <- pms * label,
+  type key       <- ms.
 
-clone import Agile_KEF as KEF with
- type key <- ms,
- type parameter <- hash,
- type secret <- pms * label.
+(* TLS master secret KEM *)
+module KEM(KEF:KEF.KEF, PMS_KEM:Inner_KEM.KEM) : Outer_KEM.KEM = {
+  fun init() : unit = {
+    PMS_KEM.init();
+    KEF.init();
+  }
 
-(* Master Secret KEM *)
-module KEM(KEF:KEF, PMS_KEM:Inner_KEM.KEM) : Outer_KEM.KEM = {
- fun init() : unit = {
-   PMS_KEM.init();
-   KEF.init();
- }
+  fun keygen() : pkey * skey = {
+    var pk : pkey;
+    var sk : skey;
+    (pk, sk) = PMS_KEM.keygen();
+    return (pk, sk);
+  }
 
- fun keygen() : pkey * skey = {
-   var pk : pkey;
-   var sk : skey;
-   (pk, sk) = PMS_KEM.keygen();
-   return (pk, sk);
- }
+  fun enc(p:version * hash, pk:pkey, t:label) : ms * ciphertext = {
+    var pms : pms;
+    var ms : ms;
+    var c : ciphertext;
+    var pv : version;
+    var h : hash;
+    (pv, h) = p;
+    (pms, c) = PMS_KEM.enc((), pk, pv);
+    ms = KEF.extract(h, (pms, t));
+    return (ms, c);
+  }
 
- fun enc(p:version * hash, pk:pkey, t:label) : ms * ciphertext = {
-   var pms : pms;
-   var ms : ms;
-   var c : ciphertext;
-   var pv : version;
-   var h : hash;
-   (pv, h) = p;
-   (pms, c) = PMS_KEM.enc((), pk, pv);
-   ms = KEF.extract(h, (pms, t));
-   return (ms, c);
- }
-
- fun dec(p:version * hash, sk:skey, t:label, c:ciphertext) : ms = {
-   var pms : pms;
-   var ms : ms;
-   var pv : version;
-   var h : hash;
-   (pv, h) = p;
-   pms = PMS_KEM.dec((), sk, pv, c);
-   ms = KEF.extract(h, (pms, t));
-   return ms;
- }
+  fun dec(p:version * hash, sk:skey, t:label, c:ciphertext) : ms = {
+    var pms : pms;
+    var ms : ms;
+    var pv : version;
+    var h : hash;
+    (pv, h) = p;
+    pms = PMS_KEM.dec((), sk, pv, c);
+    ms = KEF.extract(h, (pms, t));
+    return ms;
+  }
 }.
 
 
 (* Agile KEF in the ROM *)
-module RO_KEF : KEF = {
- var m : (hash * (pms * label), ms) map
+module RO_KEF : KEF.KEF = {
+  var m : (hash * (pms * label), ms) map
  
- fun init() : unit = {
-   m = Core.empty;
- }
+  fun init() : unit = {
+    m = Core.empty;
+  }
  
- fun extract(p:hash, s:pms * label) : ms = {
-   if (!in_dom (p, s) m) {
-     m.[(p, s)] = $Outer_KEM.key;
-   }
-   return (proj m.[(p, s)]);
- }
+  fun extract(p:hash, s:pms * label) : ms = {
+    if (!in_dom (p, s) m) m.[(p, s)] = $key;
+    return proj m.[(p, s)];
+  }
 }.
 
-lemma lossless_init : islossless RO_KEF.init.
-proof.
- by fun; wp.
-qed.
+lemma lossless_init : islossless RO_KEF.init 
+by (fun; wp).
 
-lemma lossless_extract : islossless RO_KEF.extract.
-proof.
- by fun; if => //; rnd; skip; progress; smt.
-qed. 
+lemma lossless_extract : islossless RO_KEF.extract
+by (fun; if => //; rnd; skip; smt).
 
 (* RCCA Adversary in the ROM *)
-module type Adversary(KO:KEF.Oracles, O:RCCA.Oracles) = {
- fun choose(pk:pkey) : label {* O.dec KO.extract}
- fun guess(c:ciphertext, k:ms) : bool
-}.
+import Outer_KEM.RCCA.
 
+module type Adversary(O1:KEF.Oracle, O2:Oracle) = {
+  fun choose(pk:pkey) : label {* O2.dec O1.extract}
+  fun guess(c:ciphertext, k:ms) : bool
+}.
 
 section.
 
- declare module PMS_KEM : Inner_KEM.KEM 
-   {RO_KEF, RCCA.RCCA, NR_PCA.NR_PCA, OW_PCA.OW_PCA}.
+  declare module PMS_KEM : Inner_KEM.KEM 
+    {RO_KEF, RCCA, PCA.NR_PCA, PCA.OW_PCA}.
 
- axiom lossless_dec : islossless PMS_KEM.dec.
+  (* Assumptions about the Pre-master secret KEM *)
+  axiom lossless_dec : islossless PMS_KEM.dec.
 
- (* PMS_KEM is stateless *)
- axiom stateless_pms_kem : forall (x y:glob PMS_KEM), x = y.
-
- (* Crucial *)
- axiom dec_injective_pv : forall sk pv1 pv2 c,
-   decrypt () sk pv1 c = decrypt () sk pv2 c => pv1 = pv2.
-
- axiom enc_spec_rel : forall (pk:pkey) (sk:skey) (t:version),
-   equiv [ PMS_KEM.enc ~ PMS_KEM.enc :
-    pk{1} = pk /\ t{1} = t /\ ={pk, t} /\ keypair pk sk ==>
-    ={res} /\ let (k, c) = res{1} in decrypt () sk t c = k ].
-
- axiom dec_spec_rel : forall (sk:skey) (t:version) (c:ciphertext),
-   equiv [ PMS_KEM.dec ~ PMS_KEM.dec :
-    sk{1} = sk /\ t{1} = t /\ c{1} = c /\ ={sk, t, c} ==>
-    ={res} /\ res{1} = decrypt () sk t c ].
-
- axiom dec_spec : forall (_sk:skey) (_t:version) (_c:ciphertext),
-   bd_hoare [ PMS_KEM.dec : 
-    sk = _sk /\ t = _t /\ c = _c ==> 
-    res = decrypt () _sk _t _c ] = 1%r.
-
- local module MS_KEM = KEM(RO_KEF, PMS_KEM).
-
- declare module A : Adversary
-   {RO_KEF, PMS_KEM, RCCA.RCCA, NR_PCA.NR_PCA, OW_PCA.OW_PCA}.
-
- axiom lossless_choose : 
-   forall (KO <: KEF.Oracles{A}) (O <: RCCA.Oracles{A}),
-    islossless O.dec => islossless KO.extract => islossless A(KO, O).choose.
-
- axiom lossless_guess : 
-   forall (KO <: KEF.Oracles{A}) (O <: RCCA.Oracles{A}),
-    islossless O.dec => islossless KO.extract => islossless A(KO, O).guess.
-
- import RCCA.
-
- (* Global variables in RCCA1 and RCCA2 *)
- local module V = {
-  var sk : skey
-  var keys : ms set
-  var labels : label set
-  var guess : bool
-  var t : label
-  var c : ciphertext 
-  var pms : pms
-
-  fun init() : unit = {
-    V.keys = FSet.empty;
-    V.labels = FSet.empty;
-    V.guess = false;
-    V.t = pick FSet.empty;
-    V.c = pick FSet.empty;
-    V.pms = pick FSet.empty;
-  }
- }.
-
- local module RCCA1 = {
-  var m : (hash * (pms * label), ms) map
-  var abort : bool
-
-  module O = {
-   fun extract(p:hash, s:pms * label) : ms = {
-     var pms : pms;
-     var t : label;
-     (pms, t) = s;
-     abort = abort \/ (p = snd p' /\ pms = V.pms);
-     if (!in_dom (p, (pms, t)) m) m.[(p, (pms, t))] = $Outer_KEM.key;
-     return proj m.[(p, (pms, t))];
-   }
-
-   fun dec(p:version * hash, t:label, c:ciphertext) : ms option = {
-     var pv : version;
-     var h : hash;
-     var pms : pms;
-     var k : ms;
-     var maybe_k : ms option = None;
-     if (!mem t V.labels /\ mem p P) { 
-       V.labels = add t V.labels;
-       (pv, h) = p;
-       pms = PMS_KEM.dec((), V.sk, pv, c);
-       abort = abort \/ (V.guess /\ pms = V.pms /\ t = V.t /\ c <> V.c);
-       if (!(V.guess /\ (pv, h) = p' /\ t = V.t /\ c = V.c)) {
-         if (!in_dom (h, (pms, t)) m) m.[(h, (pms, t))] = $Outer_KEM.key;
-         k = proj m.[(h, (pms, t))];
-         maybe_k = if (!mem k V.keys) then Some k else None;
-       }
-     }
-     return maybe_k;
-   }
-  }
+  (* TODO: remove this *)
+  axiom stateless_pms_kem : forall (x y:glob PMS_KEM), x = y.
   
-  module A = A(O, O)
+  pred keypair : (pkey * skey).
 
-  fun main() : bool = {
-    var b, b', valid : bool;
-    var k0, k1 : ms;
-    var pk : pkey;
-    PMS_KEM.init();
-    (pk, V.sk) = PMS_KEM.keygen();
-    V.init();
-    m = Core.empty;
-    abort = false;
-    (V.pms, V.c) = PMS_KEM.enc((), pk, fst p');
-    V.t = A.choose(pk);
-    valid = !mem V.t V.labels;
-    k0 = $Outer_KEM.key;
-    k1 = $Outer_KEM.key;
-    V.keys = add k0 (add k1 V.keys);
-    V.guess = true;
-    b' = A.guess(V.c, k0);
-    b = ${0,1};
-    return (b = b' /\ valid);
-  }
- }.
+  op decrypt : skey -> version -> ciphertext -> pms.
+  
+  (* Crucial *)
+  axiom dec_injective_pv : forall sk pv1 pv2 c,
+    decrypt sk pv1 c = decrypt sk pv2 c => pv1 = pv2.
 
- (** RCCA -> RCCA 1 **)
+  axiom keygen_rel :
+    equiv [ PMS_KEM.keygen ~ PMS_KEM.keygen : 
+      true ==> ={res} /\ keypair res{1} ].
 
- local equiv RCCA_RCCA1_extract_upto :
-   RO_KEF.extract ~ RCCA1.O.extract :
-   !RCCA1.abort{2} /\
-   ={p, s} /\
-   V.guess{2} /\
-   RCCA.sk{1} = V.sk{2} /\
-   RCCA.keys{1} = V.keys{2} /\
-   RCCA.labels{1} = V.labels{2} /\
-   eq_except RO_KEF.m{1} RCCA1.m{2} (snd p', (V.pms, V.t)){2} /\
-   in_dom (snd p', (V.pms, V.t)){2} RO_KEF.m{1} /\
-   mem (proj RO_KEF.m{1}.[(snd p', (V.pms, V.t))]){2} V.keys{2} /\
-   decrypt () V.sk{2} (fst p') V.c{2} = V.pms{2}
-   ==>
-   !RCCA1.abort{2} =>
-    ={res} /\
-    V.guess{2} /\
-    RCCA.sk{1} = V.sk{2} /\
-    RCCA.keys{1} = V.keys{2} /\
-    RCCA.labels{1} = V.labels{2} /\
-    eq_except RO_KEF.m{1} RCCA1.m{2} (snd p', (V.pms, V.t)){2} /\
-    in_dom (snd p', (V.pms, V.t)){2} RO_KEF.m{1} /\
-    mem (proj RO_KEF.m{1}.[(snd p', (V.pms, V.t))]){2} V.keys{2} /\
-    decrypt () V.sk{2} (fst p') V.c{2} = V.pms{2}.
- proof.
-  fun.
-   sp; case RCCA1.abort{2}.
-    (* aborts *)
-    if{1}; if{2}.
-     by rnd; skip; progress; smt.
-     by rnd{1}; skip; progress; smt.
-     by rnd{2}; skip; progress; smt.
-     by skip; progress; smt.
+  axiom enc_spec_rel : forall pk sk pv,
+    equiv [ PMS_KEM.enc ~ PMS_KEM.enc :
+      pk{1} = pk /\ t{1} = pv /\ ={pk, t} /\ keypair(pk, sk) ==>
+      ={res} /\ let (k, c) = res{1} in decrypt sk pv c = k ].
+  
+  axiom dec_spec_rel : forall sk pv c,
+    equiv [ PMS_KEM.dec ~ PMS_KEM.dec :
+      sk{1} = sk /\ t{1} = pv /\ c{1} = c /\ ={sk, t, c} ==>
+      ={res} /\ res{1} = decrypt sk pv c ].
+  
+  axiom dec_spec : forall _sk _pv _c,
+    bd_hoare [ PMS_KEM.dec :
+      sk = _sk /\ t = _pv /\ c = _c ==> res = decrypt _sk _pv _c ] = 1%r.
+  
+  (* TLS master secret KEM in the ROM for KEF *)
+  local module MS_KEM = KEM(RO_KEF, PMS_KEM).
+
+  (* RCCA adversary *)
+  declare module A : Adversary
+    {RO_KEF, PMS_KEM, RCCA, PCA.NR_PCA, PCA.OW_PCA}.
+
+  axiom lossless_choose : 
+    forall (O1 <: KEF.Oracle {A}) (O2 <: Oracle {A}),
+      islossless O2.dec => islossless O1.extract => islossless A(O1, O2).choose.
+
+  axiom lossless_guess : 
+    forall (O1 <: KEF.Oracle {A}) (O2 <: Oracle {A}),
+      islossless O2.dec => islossless O1.extract => islossless A(O1, O2).guess.
+
+  (* Global variables in RCCA1 and RCCA2 *)
+  local module V = {
+    var sk : skey
+    var keys : ms set
+    var labels : label set
+    var guess : bool
+    var t : label
+    var c : ciphertext 
+    var pms : pms
+  
+    fun init() : unit = {
+      keys = FSet.empty;
+      labels = FSet.empty;
+      guess = false;
+      t = pick FSet.empty;
+      c = pick FSet.empty;
+      pms = pick FSet.empty;
+    }
+  }.
+  
+  local module RCCA1 = {
+    var m : (hash * (pms * label), ms) map
+    var abort : bool
+  
+    module O1 = {
+      fun extract(p:hash, s:pms * label) : ms = {
+        var pms : pms;
+        var t : label;
+        (pms, t) = s;
+        abort = abort \/ (p = snd pp /\ pms = V.pms);
+        if (!in_dom (p, (pms, t)) m) m.[(p, (pms, t))] = $key;
+        return proj m.[(p, (pms, t))];
+      }
+    }
+  
+    module O2 = {
+      fun dec(p:version * hash, t:label, c:ciphertext) : ms option = {
+        var pv : version;
+        var h : hash;
+        var pms : pms;
+        var k : ms;
+        var maybe_k : ms option = None;
+        if (!mem t V.labels /\ mem p P) { 
+          V.labels = add t V.labels;
+          (pv, h) = p;
+          pms = PMS_KEM.dec((), V.sk, pv, c);
+          abort = abort \/ (V.guess /\ pms = V.pms /\ t = V.t /\ c <> V.c);
+          if (!(V.guess /\ (pv, h) = pp /\ t = V.t /\ c = V.c)) {
+            if (!in_dom (h, (pms, t)) m) m.[(h, (pms, t))] = $key;
+            k = proj m.[(h, (pms, t))];
+            maybe_k = if (!mem k V.keys) then Some k else None;
+          }
+        }
+        return maybe_k;
+      }
+    }
    
-    (* doesn't abort *)
-    if.
-     by progress; smt.
-     by wp; rnd; skip; progress; smt.
-
-    wp; skip; progress.
-    cut W : 
-      (p, (pms, t)){2} <>
-      (snd p', (decrypt () V.sk (fst p') V.c, V.t)){2} by smt.
-    by generalize H1; rewrite eq_except_def; smt.
- qed.
-
- local equiv RCCA_RCCA1_dec_upto :
-   RCCA(MS_KEM, A(RO_KEF)).O.dec ~ RCCA1.O.dec :
-   !RCCA1.abort{2} /\
-   ={p, t, c} /\
-   V.guess{2} /\
-   RCCA.sk{1} = V.sk{2} /\
-   RCCA.keys{1} = V.keys{2} /\
-   RCCA.labels{1} = V.labels{2} /\
-   eq_except RO_KEF.m{1} RCCA1.m{2} (snd p', (V.pms, V.t)){2} /\
-   in_dom (snd p', (V.pms, V.t)){2} RO_KEF.m{1} /\
-   mem (proj RO_KEF.m{1}.[(snd p', (V.pms, V.t))]){2} V.keys{2} /\
-   decrypt () V.sk{2} (fst p') V.c{2} = V.pms{2}
-   ==>
-   !RCCA1.abort{2} =>
-    ={res} /\
+   module A = A(O1, O2)
+  
+    fun main() : bool = {
+     var b, b', valid : bool;
+     var k0, k1 : ms;
+     var pk : pkey;
+     PMS_KEM.init();
+     (pk, V.sk) = PMS_KEM.keygen();
+     V.init();
+     m = Core.empty;
+     abort = false;
+     (V.pms, V.c) = PMS_KEM.enc((), pk, fst pp);
+     V.t = A.choose(pk);
+     valid = !mem V.t V.labels;
+     k0 = $key;
+     k1 = $key;
+     V.keys = add k0 (add k1 V.keys);
+     V.guess = true;
+     b' = A.guess(V.c, k0);
+     b = ${0,1};
+     return (b = b' /\ valid);
+   }
+  }.
+  
+  (** RCCA -> RCCA 1 **)
+  local equiv RCCA_RCCA1_extract_upto :
+    RO_KEF.extract ~ RCCA1.O1.extract :
+    !RCCA1.abort{2} /\
+    ={p, s} /\
     V.guess{2} /\
-    RCCA.sk{1} = V.sk{2} /\
-    RCCA.keys{1} = V.keys{2} /\
-    RCCA.labels{1} = V.labels{2} /\
-    eq_except RO_KEF.m{1} RCCA1.m{2} (snd p', (V.pms, V.t)){2} /\
-    in_dom (snd p', (V.pms, V.t)){2} RO_KEF.m{1} /\
-    mem (proj RO_KEF.m{1}.[(snd p', (V.pms, V.t))]){2} V.keys{2} /\
-    decrypt () V.sk{2} (fst p') V.c{2} = V.pms{2}.
- proof.
-  fun.
-  sp; if => //.  
-  wp; inline KEM(RO_KEF, PMS_KEM).dec.
-  seq 7 3 : 
-   ((decrypt () RCCA.sk pv c0 = pms){1} /\
-    maybe_k{1} = None /\
-    sk{1} = RCCA.sk{1} /\ c0{1} = c{2} /\ t0{1} = t{2} /\
-    ={maybe_k, pms, pv, h, p, t, c} /\
-    !RCCA1.abort{2} /\ 
+    W.sk{1} = V.sk{2} /\
+    W.keys{1} = V.keys{2} /\
+    W.labels{1} = V.labels{2} /\
+    eq_except RO_KEF.m{1} RCCA1.m{2} (snd pp, (V.pms, V.t)){2} /\
+    in_dom (snd pp, (V.pms, V.t)){2} RO_KEF.m{1} /\
+    mem (proj RO_KEF.m{1}.[(snd pp, (V.pms, V.t))]){2} V.keys{2} /\
+    decrypt V.sk{2} (fst pp) V.c{2} = V.pms{2}
+    ==>
+    !RCCA1.abort{2} =>
+      ={res} /\
+      V.guess{2} /\
+      W.sk{1} = V.sk{2} /\
+      W.keys{1} = V.keys{2} /\
+      W.labels{1} = V.labels{2} /\
+      eq_except RO_KEF.m{1} RCCA1.m{2} (snd pp, (V.pms, V.t)){2} /\
+      in_dom (snd pp, (V.pms, V.t)){2} RO_KEF.m{1} /\
+      mem (proj RO_KEF.m{1}.[(snd pp, (V.pms, V.t))]){2} V.keys{2} /\
+      decrypt V.sk{2} (fst pp) V.c{2} = V.pms{2}.
+  proof.
+    fun.
+    sp; case RCCA1.abort{2}.
+      (* aborts *)
+      if{1}; if{2}.
+        by rnd; skip; smt.
+        by rnd{1}; skip; smt.
+        by rnd{2}; skip; smt.
+        by skip; smt.     
+      (* doesn't abort *)
+      if.
+        by smt.
+        by wp; rnd; skip; progress; smt.    
+      wp; skip; progress.
+      cut W : 
+        (p, (pms, t)){2} <>
+        (snd pp, (decrypt V.sk (fst pp) V.c, V.t)){2} by smt.
+      by generalize H1; rewrite eq_except_def; smt.
+  qed.
+  
+  local equiv RCCA_RCCA1_dec_upto :
+    RCCA(MS_KEM, A(RO_KEF)).O.dec ~ RCCA1.O2.dec :
+    !RCCA1.abort{2} /\
+    ={p, t, c} /\
     V.guess{2} /\
-    RCCA.sk{1} = V.sk{2} /\
-    RCCA.keys{1} = V.keys{2} /\
-    RCCA.labels{1} = V.labels{2} /\
-    eq_except RO_KEF.m{1} RCCA1.m{2} (snd p', (V.pms, V.t)){2} /\
-    in_dom (snd p', (V.pms, V.t)){2} RO_KEF.m{1} /\
-    mem (proj RO_KEF.m{1}.[(snd p', (V.pms, V.t))]){2} V.keys{2} /\
-    decrypt () V.sk{2} (fst p') V.c{2} = V.pms{2}).
-   sp; exists * sk{1}, pv{1}, c0{1}; elim *; intros sk pv c.
-   by call (dec_spec_rel sk pv c); wp.
+    W.sk{1} = V.sk{2} /\
+    W.keys{1} = V.keys{2} /\
+    W.labels{1} = V.labels{2} /\
+    eq_except RO_KEF.m{1} RCCA1.m{2} (snd pp, (V.pms, V.t)){2} /\
+    in_dom (snd pp, (V.pms, V.t)){2} RO_KEF.m{1} /\
+    mem (proj RO_KEF.m{1}.[(snd pp, (V.pms, V.t))]){2} V.keys{2} /\
+    decrypt V.sk{2} (fst pp) V.c{2} = V.pms{2}
+    ==>
+    !RCCA1.abort{2} =>
+      ={res} /\
+      V.guess{2} /\
+      W.sk{1} = V.sk{2} /\
+      W.keys{1} = V.keys{2} /\
+      W.labels{1} = V.labels{2} /\
+      eq_except RO_KEF.m{1} RCCA1.m{2} (snd pp, (V.pms, V.t)){2} /\
+      in_dom (snd pp, (V.pms, V.t)){2} RO_KEF.m{1} /\
+      mem (proj RO_KEF.m{1}.[(snd pp, (V.pms, V.t))]){2} V.keys{2} /\
+      decrypt V.sk{2} (fst pp) V.c{2} = V.pms{2}.
+  proof.
+    fun.
+    sp; if => //.  
+    wp; inline KEM(RO_KEF, PMS_KEM).dec.
+    seq 7 3 : 
+      ((decrypt W.sk pv c0 = pms){1} /\
+       maybe_k{1} = None /\
+       sk{1} = W.sk{1} /\ c0{1} = c{2} /\ t0{1} = t{2} /\
+       ={maybe_k, pms, pv, h, p, t, c} /\
+       !RCCA1.abort{2} /\ 
+       V.guess{2} /\
+       W.sk{1} = V.sk{2} /\
+       W.keys{1} = V.keys{2} /\
+       W.labels{1} = V.labels{2} /\
+       eq_except RO_KEF.m{1} RCCA1.m{2} (snd pp, (V.pms, V.t)){2} /\
+       in_dom (snd pp, (V.pms, V.t)){2} RO_KEF.m{1} /\
+       mem (proj RO_KEF.m{1}.[(snd pp, (V.pms, V.t))]){2} V.keys{2} /\
+       decrypt V.sk{2} (fst pp) V.c{2} = V.pms{2}).
+      sp; exists * sk{1}, pv{1}, c0{1}; elim *; intros sk pv c.
+      by call (dec_spec_rel sk pv c); wp.
+   
+      wp; sp; case RCCA1.abort{2}.
+        (* aborts *)
+        call{1} (_:true ==> true); first by apply lossless_extract.
+        if{2}.
+          if{2}.
+            by wp; rnd{2}; skip; smt.
+            by wp; skip; smt.
+          by skip; smt.
+   
+        (* doesn't abort *)
+        inline{1} RO_KEF.extract.
+        if{2}.
+          wp; sp; if.
+            by progress; cut W :
+              (snd pp, (decrypt V.sk (fst pp) V.c, V.t)){2} <>
+              (h, (decrypt V.sk pv c, t)){2}; smt.   
+            by rnd; skip; progress; smt.
+      
+         skip; progress.
+         cut W :
+           (snd pp, (decrypt V.sk (fst pp) V.c, V.t)){2} <>
+           (h, (decrypt V.sk pv c, t)){2} by smt.
+         by generalize H1; rewrite eq_except_def; smt.
+   
+      wp; sp; if{1}.
+        by rnd{1}; skip; smt.
+        by skip; smt.
+  qed.
+  
+  local lemma RCCA_lossless_dec : islossless RCCA(MS_KEM, A(RO_KEF)).O.dec.
+  proof.
+    fun.
+    sp; if => //.
+    inline KEM(RO_KEF, PMS_KEM).dec; wp; sp.
+    seq 1 : true => //.
+      by call (_:true) => //; apply lossless_dec.
+      by call (_:true ==> true) => //; apply lossless_extract.
+  qed.
 
-   wp; sp; case RCCA1.abort{2}.
-    (* aborts *)
-    call{1} (_:true ==> true); first by apply lossless_extract.
-    if{2}.
-     if{2}.
-      by wp; rnd{2}; skip; smt.
-      by wp; skip; progress; smt.
-     by skip; progress; smt.
- 
-   (* doesn't abort *)
-   inline{1} RO_KEF.extract.
-   if{2}.
-    wp; sp; if.
-     progress; try smt.
-     cut W :
-      (snd p', (decrypt () V.sk (fst p') V.c, V.t)){2} <>
-      (h, (decrypt () V.sk pv c, t)){2}; smt.
-
-     by rnd; skip; progress; smt.
-    
-     skip; progress.
-     cut W :
-      (snd p', (decrypt () V.sk (fst p') V.c, V.t)){2} <>
-      (h, (decrypt () V.sk pv c, t)){2} by smt.
-     by generalize H1; rewrite eq_except_def; smt.
-
-   wp; sp; if{1}.
-    by rnd{1}; skip; progress; smt.
-    by skip; progress; smt.
- qed.
-
- local lemma RCCA_lossless_dec : islossless RCCA(MS_KEM, A(RO_KEF)).O.dec.
- proof.
-  fun.
-  sp; if => //.
-  inline KEM(RO_KEF, PMS_KEM).dec; wp; sp.
-  seq 1 : true => //.
-   by call (_:true) => //; apply lossless_dec.
-   by call (_:true ==> true) => //; apply lossless_extract.
- qed.
-
- local lemma RCCA1_dec_preserves_abort : 
-   bd_hoare [ RCCA1.O.dec : RCCA1.abort ==> RCCA1.abort ] = 1%r.
- proof.
-  fun.
-  sp; if => //; wp.
-  seq 3 : RCCA1.abort => //.
-   by call (_:RCCA1.abort); [apply lossless_dec | wp]. 
-   sp; if => //; wp; if. 
-    by rnd; skip; smt.
-    by wp; skip; smt.
-   by bd_hoare; call (_:RCCA1.abort); wp.
- qed.
-
- local equiv RCCA_RCCA1_extract :
-   RO_KEF.extract ~ RCCA1.O.extract :
-   !RCCA1.abort{2} /\
-   ={p, s} /\ 
-   !V.guess{2} /\
-   RO_KEF.m{1} = RCCA1.m{2} /\
-   RCCA.sk{1} = V.sk{2} /\
-   RCCA.keys{1} = V.keys{2} /\
-   RCCA.labels{1} = V.labels{2} /\
-   decrypt () V.sk{2} (fst p') V.c{2} = V.pms{2} /\
-   (forall t,
-    in_dom (snd p', (V.pms, t)) RCCA1.m => 
-    RCCA1.abort \/ mem t V.labels){2}
-   ==>
-   !RCCA1.abort{2} =>
-    ={res} /\ 
-    !V.guess{2} /\
-    RO_KEF.m{1} = RCCA1.m{2} /\
-    RCCA.sk{1} = V.sk{2} /\
-    RCCA.keys{1} = V.keys{2} /\
-    RCCA.labels{1} = V.labels{2} /\
-    decrypt () V.sk{2} (fst p') V.c{2} = V.pms{2} /\
-    (forall t,
-     in_dom (snd p', (V.pms, t)) RCCA1.m => 
-     RCCA1.abort \/ mem t V.labels){2}.
- proof.
-  fun.
-  sp; case RCCA1.abort{2}.
-   by if{1}; if{2}; try rnd{1}; try rnd{2}; skip; progress; smt.
-   if => //.
-    by rnd; skip; progress; smt. 
-    by skip; progress; smt.
- qed.
-
- local equiv RCCA_RCCA1_dec :
-   RCCA(MS_KEM, A(RO_KEF)).O.dec ~ RCCA1.O.dec :
-   !RCCA1.abort{2} /\
-   ={p, t, c} /\ 
-   !V.guess{2} /\
-   RO_KEF.m{1} = RCCA1.m{2} /\
-   RCCA.sk{1} = V.sk{2} /\
-   RCCA.keys{1} = V.keys{2} /\
-   RCCA.labels{1} = V.labels{2} /\
-   (decrypt () V.sk (fst p') V.c = V.pms){2} /\
-   (forall t,
-    in_dom (snd p', (V.pms, t)) RCCA1.m => 
-    RCCA1.abort \/ mem t V.labels){2}
-   ==>
-   !RCCA1.abort{2} =>
-    ={res} /\ 
-    !V.guess{2} /\
-    RO_KEF.m{1} = RCCA1.m{2} /\
-    RCCA.sk{1} = V.sk{2} /\
-    RCCA.keys{1} = V.keys{2} /\
-    RCCA.labels{1} = V.labels{2} /\
-    (decrypt () V.sk (fst p') V.c = V.pms){2} /\
-    (forall t,
-     in_dom (snd p', (V.pms, t)) RCCA1.m => 
-     RCCA1.abort \/ mem t V.labels){2}.
- proof.
-  fun.
-  sp; if => //.
-  inline KEM(RO_KEF, PMS_KEM).dec.
-  seq 7 3 :
-    (!RCCA1.abort{2} /\
-     !V.guess{2} /\
-     ={maybe_k, pms, p, t, c} /\
-     (pms = decrypt () V.sk pv c){2} /\
-     (pv{2}, h{2}) = p{2} /\
-     t0{1} = t{1} /\
-     p0{1} = p{1} /\
-     sk{1} = RCCA.sk{1} /\
-     c0{1} = c{1} /\
-     (pv, h){1} = p0{1} /\
-     mem t{2} V.labels{2} /\
-     mem p{2} P /\
-     RO_KEF.m{1} = RCCA1.m{2} /\
-     RCCA.sk{1} = V.sk{2} /\
-     RCCA.keys{1} = V.keys{2} /\
-     RCCA.labels{1} = V.labels{2} /\
-     (decrypt () V.sk (fst p') V.c = V.pms){2} /\
-     (forall t,
-     in_dom (snd p', (V.pms, t)) RCCA1.m => 
-     RCCA1.abort \/ mem t V.labels){2}).
-   sp; exists * sk{1}, pv{1}, c0{1}; elim *; intros sk pv c.
-   by call (dec_spec_rel sk pv c); skip; progress; smt.
-
-   inline{1} RO_KEF.extract; wp; sp.
-   if{2}.
-    if => //.
-     by wp; rnd; skip; progress; smt.
-     by wp; skip; progress; smt.
-
-    if{1}.
-     by rnd{1}; skip; progress; smt.
-     by skip; progress; smt.
- qed.
-
- (* TODO: workaround for transitivity below *) 
- local module M = RCCA(MS_KEM, A(RO_KEF)).
-
- local equiv RCCA_RCCA1 :
-   RCCA(MS_KEM, A(RO_KEF)).main ~ RCCA1.main : true ==> !RCCA1.abort{2} => ={res}.
- proof.
-  fun.
-  swap{1} 9 -3; swap{2} 14 -6.
-  inline KEM(RO_KEF, PMS_KEM).enc.
-
-  (* Workaround to swap PMS_KEM.enc *)
-  transitivity {1} {
-   MS_KEM.init();
-   (RCCA.pk, RCCA.sk) = MS_KEM.keygen();
-   RCCA.keys = FSet.empty;
-   RCCA.labels = FSet.empty;
-   (pms, c) = PMS_KEM.enc((), RCCA.pk, fst p');
-   t = M.A.choose(RCCA.pk);
-   b = ${0,1};
-   valid = !mem t RCCA.labels;
-   k0 = RO_KEF.extract(snd p', (pms, t));
-   k1 = $Outer_KEM.key;
-   RCCA.keys = add k0 (add k1 RCCA.keys);
-   b'= M.A.guess(c, b ? k1 : k0);
-  }
-  (true ==> ={b, b', valid, RCCA1.abort})
-  (true ==> !RCCA1.abort{2} => (b = b' /\ valid){1} = (b = b' /\ valid){2}) => //.
-  swap{1} 6 6; swap{1} 6 6.
-  inline RO_KEF.extract MS_KEM.init KEM(RO_KEF, PMS_KEM).init;
-  eqobs_in; wp; rnd.
-  admit (* swap{2} 6 1.*).
-  (*********************************)
-
-  seq 7 8 : 
-   (={b} /\
-    pms{1} = V.pms{2} /\
-    c{1} = V.c{2} /\
-    (!RCCA1.abort{2} =>
-     ={glob A} /\
-     t{1} = V.t{2} /\
-     RO_KEF.m{1} = RCCA1.m{2} /\
-     RCCA.sk{1} = V.sk{2} /\
-     RCCA.keys{1} = V.keys{2} /\
-     RCCA.labels{1} = V.labels{2} /\
-     (decrypt () V.sk (fst p') V.c = V.pms){2} /\
-     (forall t,
-      in_dom (snd p', (V.pms, t)) RCCA1.m => mem t V.labels){2})).
-   wp; rnd; simplify.
-   call (_:RCCA1.abort,
-    !V.guess{2} /\
-    RO_KEF.m{1} = RCCA1.m{2} /\
-    RCCA.sk{1} = V.sk{2} /\
-    RCCA.keys{1} = V.keys{2} /\
-    RCCA.labels{1} = V.labels{2} /\
-    (decrypt () V.sk (fst p') V.c = V.pms){2} /\
-    (forall t,
-     in_dom (snd p', (V.pms, t)) RCCA1.m => 
-     RCCA1.abort \/ mem t V.labels){2}).
-    by apply lossless_choose.
-    by apply RCCA_RCCA1_dec.
-    by progress; apply RCCA_lossless_dec.
-    by apply RCCA1_dec_preserves_abort.
-    by apply RCCA_RCCA1_extract.
-    by progress; apply lossless_extract.
-    by progress; fun; sp; if; try rnd; skip; smt.
-  seq 2 2 : (RCCA.pk{1} = pk{2} /\ RCCA.sk{1} = V.sk{2} /\ RO_KEF.m{1} = Core.empty).
-  inline MS_KEM.init RO_KEF.init MS_KEM.keygen.
-  wp; call (_:true); wp; call (_:true); skip; progress.
-  exists * V.sk{2}, pk{2}; elim *; intros sk pk.
-  call (enc_spec_rel pk sk (fst p')).
-  by inline V.init; wp; skip; progress; smt.
-
-  inline RO_KEF.extract; wp; sp.
-  case RCCA1.abort{2}.
-   (* abort *)
-   call (_:RCCA1.abort, RCCA1.abort{2}).
-    by apply lossless_guess.
-    by exfalso; smt.
-    by progress; apply RCCA_lossless_dec.
-    by apply RCCA1_dec_preserves_abort.
-    by exfalso; smt.
-    by progress; apply lossless_extract.
-    by progress; fun; sp; if; try rnd; skip; smt.
-   wp; rnd; wp; if{1}.
-    by rnd; skip; progress; smt.
-    by rnd{2}; skip; progress; smt.
-
-  (* !abort *)
-  case valid{1}.
-   (* valid *)
-   rcondt{1} 1; first by intros _; skip; smt.
-   call (_:RCCA1.abort,
-    V.guess{2} /\
-    RCCA.sk{1} = V.sk{2} /\
-    RCCA.keys{1} = V.keys{2} /\
-    RCCA.labels{1} = V.labels{2} /\
-    eq_except RO_KEF.m{1} RCCA1.m{2} (snd p', (V.pms, V.t)){2} /\
-    in_dom (snd p', (V.pms, V.t)){2} RO_KEF.m{1} /\
-    mem (proj RO_KEF.m{1}.[(snd p', (V.pms, V.t))]){2} V.keys{2} /\
-    decrypt () V.sk{2} (fst p') V.c{2} = V.pms{2}).
-   by apply lossless_guess.
-   by apply RCCA_RCCA1_dec_upto.
-   by progress; apply RCCA_lossless_dec.
-   by apply RCCA1_dec_preserves_abort.
-   by apply RCCA_RCCA1_extract_upto.
-   by progress; apply lossless_extract.
-   by intros _; fun; sp; if; try rnd; skip; smt.
-   wp; case b{1}.
-    by swap{2} 1; rnd; wp; rnd; skip; progress; smt.
-    by rnd; wp; rnd; skip; progress; smt.
-
-   (* !abort /\ !valid *)  
-   call{1} (_:true ==> true).
-   apply (lossless_guess RO_KEF (<:RCCA(MS_KEM, A(RO_KEF)).O)).
-    (* lossless RCCA.O.dec *)
+  local lemma RCCA1_lossless_dec : islossless RCCA1.O2.dec.
+  proof.
     fun.
     sp; if => //.
     sp; seq 1 : true => //.
-     call (_:true) => //.
-     call (_:true).
-      by if; try rnd; skip; smt.
-      by call (_:true); [apply lossless_dec | wp].
-      by wp.
-    (* lossless RCCA1.O.extract *)      
-    by fun; sp; if => //; rnd; skip; smt.
-   call{2} (_:true ==> true).
-   apply (lossless_guess RCCA1.O RCCA1.O).
-    (* lossless RCCA1.O.dec *)
-    fun.
-     sp; if => //.
-     sp; seq 1 : true => //.
       by call (_:true); first by apply lossless_dec.
       sp; if => //.
-      by if => //; wp; try rnd; skip; smt.
-    (* lossless RCCA1.O.extract *)      
-    by fun; sp; if => //; rnd; skip; smt.
+        by if => //; wp; try rnd; skip; smt.  
+  qed.
 
-   wp; rnd; wp; if{1}.
-    by rnd; skip; progress; smt.
-    by rnd{2}; skip; smt.
- qed.
-
- local lemma Pr_RCCA1_res : forall &m, Pr[RCCA1.main() @ &m : res] <= 1%r / 2%r.
- proof.
-  intros &m; bdhoare_deno (_:true) => //. 
-  fun.
-  rnd; simplify; call (_:true).
-   (* lossless RCCA1.O.dec *)
-   fun; sp; if => //.
-   (* lossless RCCA1.O.extract *)      
-   by fun; sp; if => //; rnd; skip; smt.
-
-  wp; rnd; rnd; wp; call (_:true).
-   (* lossless RCCA1.O.dec *)
-   fun; sp; if => //.
-   (* lossless RCCA1.O.extract *)      
-   by fun; sp; if => //; rnd; skip; smt.
-
-  inline V.init.
-  call (_:true); wp; call (_:true); wp; call (_:true).
-  by skip; progress; try rewrite Bool.Dbool.mu_def; smt.
- qed.
-
- local lemma Pr_RCCA_RCCA1 : forall &m,
-   Pr[RCCA(KEM(RO_KEF, PMS_KEM), A(RO_KEF)).main() @ &m : res] <=
-   1%r / 2%r + Pr[RCCA1.main() @ &m : RCCA1.abort].
- proof.
-  intros &m.
-  apply (Trans _ (Pr[RCCA1.main() @ &m : res \/ RCCA1.abort])).
-  equiv_deno RCCA_RCCA1; smt.  
-  rewrite Pr mu_or; smt.
- qed.
-
-
- (** RCCA1 -> RCCA2 **)
-
- op find_dec sk (m:(hash * (pms * label), ms) map) pv c h t = 
-  in_dom (h, (decrypt () sk pv c, t)) m.
-
- op find_ext sk (d:(label, (ms * version * hash * ciphertext)) map) h pms t = 
-  in_dom t d /\ 
-  let (k, pv, h', c) = proj d.[t] in h = h' /\ decrypt () sk pv c = pms.
-
- local module RCCA2 = {
-  var m : (hash * (pms * label), ms) map
-  var d : (label, (ms * version * hash * ciphertext)) map
-
-  module O = {
-   fun extract(p:hash, s:pms * label) : ms = {
-     var k : ms;
-     var pms : pms;
-     var t : label;
-     (pms, t) = s;
-     if (!in_dom (p, (pms, t)) m) {
-       if (find_ext V.sk d p pms t) {
-         k = let (ms, pv, h, c) = proj d.[t] in ms;
-       }
-       else k = $Outer_KEM.key;
-       m.[(p, (pms, t))] = k;
-     }
-     else {
-       k = proj m.[(p, (pms, t))];
-     }
-     return k;
-   }
-
-   fun dec(p:version * hash, t:label, c:ciphertext) : ms option = {
-     var pv : version;
-     var h : hash;
-     var k : ms;
-     var maybe_k : ms option = None;
-     if (!mem t V.labels /\ mem p P) { 
-       V.labels = add t V.labels;
-       (pv, h) = p;
-       if (!(V.guess /\ (pv, h) = p' /\ t = V.t /\ V.c = c)) {
-         if (find_dec V.sk m pv c h t) {
-           k = proj m.[(h, (decrypt () V.sk pv c, t))];
-         }
-         else {
-           k = $Outer_KEM.key;
-         }
-         d.[t] = (k, pv, h, c);
-         maybe_k = if (!mem k V.keys) then Some k else None;
-       }
-     }
-     return maybe_k;
-   }
-  }
+  local lemma RCCA1_dec_preserves_abort : 
+    bd_hoare [ RCCA1.O2.dec : RCCA1.abort ==> RCCA1.abort ] = 1%r.
+  proof.
+    fun.
+    sp; if => //; wp.
+    seq 3 : RCCA1.abort => //.
+     by call (_:RCCA1.abort); [apply lossless_dec | wp]. 
+     sp; if => //; wp; if. 
+       by rnd; skip; smt.
+       by wp; skip; smt.
+     by bd_hoare; call (_:RCCA1.abort); wp.
+  qed.
   
-  module A = A(O, O)
+  local equiv RCCA_RCCA1_extract :
+    RO_KEF.extract ~ RCCA1.O1.extract :
+    !RCCA1.abort{2} /\
+    ={p, s} /\ 
+    !V.guess{2} /\
+    RO_KEF.m{1} = RCCA1.m{2} /\
+    W.sk{1} = V.sk{2} /\
+    W.keys{1} = V.keys{2} /\
+    W.labels{1} = V.labels{2} /\
+    decrypt V.sk{2} (fst pp) V.c{2} = V.pms{2} /\
+    (forall t,
+     in_dom (snd pp, (V.pms, t)) RCCA1.m => 
+     RCCA1.abort \/ mem t V.labels){2}
+    ==>
+    !RCCA1.abort{2} =>
+      ={res} /\ 
+      !V.guess{2} /\
+      RO_KEF.m{1} = RCCA1.m{2} /\
+      W.sk{1} = V.sk{2} /\
+      W.keys{1} = V.keys{2} /\
+      W.labels{1} = V.labels{2} /\
+      decrypt V.sk{2} (fst pp) V.c{2} = V.pms{2} /\
+      (forall t,
+       in_dom (snd pp, (V.pms, t)) RCCA1.m => 
+       RCCA1.abort \/ mem t V.labels){2}.
+  proof.
+    fun.
+    sp; case RCCA1.abort{2}.
+      by if{1}; if{2}; try rnd{1}; try rnd{2}; skip; smt.
+      if => //.
+        by rnd; skip; smt. 
+        by skip; smt.
+  qed.
+  
+  local equiv RCCA_RCCA1_dec :
+    RCCA(MS_KEM, A(RO_KEF)).O.dec ~ RCCA1.O2.dec :
+    !RCCA1.abort{2} /\
+    ={p, t, c} /\ 
+    !V.guess{2} /\
+    RO_KEF.m{1} = RCCA1.m{2} /\
+    W.sk{1} = V.sk{2} /\
+    W.keys{1} = V.keys{2} /\
+    W.labels{1} = V.labels{2} /\
+    (decrypt V.sk (fst pp) V.c = V.pms){2} /\
+    (forall t,
+     in_dom (snd pp, (V.pms, t)) RCCA1.m => 
+     RCCA1.abort \/ mem t V.labels){2}
+    ==>
+    !RCCA1.abort{2} =>
+      ={res} /\ 
+      !V.guess{2} /\
+      RO_KEF.m{1} = RCCA1.m{2} /\
+      W.sk{1} = V.sk{2} /\
+      W.keys{1} = V.keys{2} /\
+      W.labels{1} = V.labels{2} /\
+      (decrypt V.sk (fst pp) V.c = V.pms){2} /\
+      (forall t,
+       in_dom (snd pp, (V.pms, t)) RCCA1.m => 
+       RCCA1.abort \/ mem t V.labels){2}.
+  proof.
+    fun.
+    sp; if => //.
+    inline KEM(RO_KEF, PMS_KEM).dec.
+    seq 7 3 :
+     (!RCCA1.abort{2} /\
+      !V.guess{2} /\
+      ={maybe_k, pms, p, t, c} /\
+      (pms = decrypt V.sk pv c){2} /\
+      (pv{2}, h{2}) = p{2} /\
+      t0{1} = t{1} /\
+      p0{1} = p{1} /\
+      sk{1} = W.sk{1} /\
+      c0{1} = c{1} /\
+      (pv, h){1} = p0{1} /\
+      mem t{2} V.labels{2} /\
+      mem p{2} P /\
+      RO_KEF.m{1} = RCCA1.m{2} /\
+      W.sk{1} = V.sk{2} /\
+      W.keys{1} = V.keys{2} /\
+      W.labels{1} = V.labels{2} /\
+      (decrypt V.sk (fst pp) V.c = V.pms){2} /\
+      (forall t, 
+         in_dom (snd pp, (V.pms, t)) RCCA1.m => 
+         RCCA1.abort \/ mem t V.labels){2}).
+      sp; exists * sk{1}, pv{1}, c0{1}; elim *; intros sk pv c.
+      by call (dec_spec_rel sk pv c); skip; progress; smt.
+  
+      inline{1} RO_KEF.extract; wp; sp.
+      if{2}.
+        if => //.
+          by wp; rnd; skip; progress; smt.
+          by wp; skip; progress; smt.
+        if{1}.
+          by rnd{1}; skip; progress; smt.
+          by skip; progress; smt.
+  qed.
+  
+  (* TODO: workaround for transitivity below *) 
+  local module M = RCCA(MS_KEM, A(RO_KEF)).
+  
+  local equiv RCCA_RCCA1 :
+    RCCA(MS_KEM, A(RO_KEF)).main ~ RCCA1.main : 
+      true ==> !RCCA1.abort{2} => ={res}.
+  proof.
+    fun.
+    swap{1} 9 -3; swap{2} 14 -6.
+    inline KEM(RO_KEF, PMS_KEM).enc.   
+    (* Workaround to swap PMS_KEM.enc *)
+    transitivity{1} {
+      MS_KEM.init();
+      (W.pk, W.sk) = MS_KEM.keygen();
+      W.keys = FSet.empty;
+      W.labels = FSet.empty;
+      (pms, c) = PMS_KEM.enc((), W.pk, fst pp);
+      t = M.A.choose(W.pk);
+      b = ${0,1};
+      valid = !mem t W.labels;
+      k0 = RO_KEF.extract(snd pp, (pms, t));
+      k1 = $key;
+      W.keys = add k0 (add k1 W.keys);
+      b'= M.A.guess(c, b ? k1 : k0);
+    }
+    (true ==> ={b, b', valid})
+    (true ==> !RCCA1.abort{2} => (b = b' /\ valid){1} = (b = b' /\ valid){2}) => //.
+    call (_: ={glob W, RO_KEF.m}).
+      by fun; eqobs_in; progress; smt.
+      by fun; eqobs_in.
+      wp; rnd; wp.
+    call (_: ={glob W, RO_KEF.m}); first by eqobs_in.
+    inline MS_KEM.init KEM(RO_KEF, PMS_KEM).init.
+    swap{1} 7 6; swap{1} 7 6; wp; rnd.
+    swap{1} 9 2; swap{1} [7..9] -2; wp.
+    seq 8 5 : (={glob W, RO_KEF.m} /\ pk{1} = W.pk{2} /\ (pv,h){1} = pp).
+    inline RO_KEF.init; wp; call (_:true).
+      by simplify; eqobs_in; smt.
+    wp; call (_:true); skip; progress.
+    seq 2 2 : 
+      (={glob A, glob W, RO_KEF.m, t, pms} /\ 
+       c0{1} = c{2} /\ (pv, h){1} = pp).
+    admit.
+    skip; smt.
+    (*********************************)   
+    seq 7 8 : 
+     (={b} /\
+      pms{1} = V.pms{2} /\
+      c{1} = V.c{2} /\
+      (!RCCA1.abort{2} =>
+       ={glob A} /\
+       t{1} = V.t{2} /\
+       RO_KEF.m{1} = RCCA1.m{2} /\
+       W.sk{1} = V.sk{2} /\
+       W.keys{1} = V.keys{2} /\
+       W.labels{1} = V.labels{2} /\
+       (decrypt V.sk (fst pp) V.c = V.pms){2} /\
+       (forall t,
+        in_dom (snd pp, (V.pms, t)) RCCA1.m => mem t V.labels){2})).
+      wp; rnd; simplify.
+      call (_:RCCA1.abort,
+        !V.guess{2} /\
+        RO_KEF.m{1} = RCCA1.m{2} /\
+        W.sk{1} = V.sk{2} /\
+        W.keys{1} = V.keys{2} /\
+        W.labels{1} = V.labels{2} /\
+        (decrypt V.sk (fst pp) V.c = V.pms){2} /\
+        (forall t,
+         in_dom (snd pp, (V.pms, t)) RCCA1.m => 
+         RCCA1.abort \/ mem t V.labels){2}).
+      by apply lossless_choose.
+      by apply RCCA_RCCA1_dec.
+      by progress; apply RCCA_lossless_dec.
+      by apply RCCA1_dec_preserves_abort.
+      by apply RCCA_RCCA1_extract.
+      by progress; apply lossless_extract.
+      by progress; fun; sp; if; try rnd; skip; smt. 
+      seq 2 2 : 
+       (W.pk{1} = pk{2} /\ W.sk{1} = V.sk{2} /\ 
+        RO_KEF.m{1} = Core.empty /\ keypair(W.pk, W.sk){1}).
+        inline MS_KEM.init RO_KEF.init MS_KEM.keygen; wp.
+        by call keygen_rel; wp; call (_:true).
+        inline V.init; sp.
+        exists * V.sk{2}, pk{2}; elim *; intros sk pk.
+        by call (enc_spec_rel pk sk (fst pp)); skip; smt.
+      inline RO_KEF.extract; wp; sp.
+      case RCCA1.abort{2}.
+        (* abort *)
+        call (_:RCCA1.abort, RCCA1.abort{2}).
+          by apply lossless_guess.
+          by exfalso; smt.
+          by progress; apply RCCA_lossless_dec.
+          by apply RCCA1_dec_preserves_abort.
+          by exfalso; smt.
+          by progress; apply lossless_extract.
+          by progress; fun; sp; if; try rnd; skip; smt.
+        wp; rnd; wp; if{1}.
+          by rnd; skip; smt.
+          by rnd{2}; skip; smt.   
+        (* !abort *)
+        case valid{1}.
+          (* valid *)
+          rcondt{1} 1; first by intros _; skip; smt.
+          call (_:RCCA1.abort,
+           V.guess{2} /\
+           W.sk{1} = V.sk{2} /\
+           W.keys{1} = V.keys{2} /\
+           W.labels{1} = V.labels{2} /\
+           eq_except RO_KEF.m{1} RCCA1.m{2} (snd pp, (V.pms, V.t)){2} /\
+           in_dom (snd pp, (V.pms, V.t)){2} RO_KEF.m{1} /\
+           mem (proj RO_KEF.m{1}.[(snd pp, (V.pms, V.t))]){2} V.keys{2} /\
+           decrypt V.sk{2} (fst pp) V.c{2} = V.pms{2}).
+          by apply lossless_guess.
+          by apply RCCA_RCCA1_dec_upto.
+          by progress; apply RCCA_lossless_dec.
+          by apply RCCA1_dec_preserves_abort.
+          by apply RCCA_RCCA1_extract_upto.
+          by progress; apply lossless_extract.
+          by intros _; fun; sp; if; try rnd; skip; smt.
+          wp; case b{1}.
+            by swap{2} 1; rnd; wp; rnd; skip; progress; smt.
+            by rnd; wp; rnd; skip; progress; smt.
+   
+          (* !abort /\ !valid *)  
+          call{1} (_:true ==> true).
+            apply (lossless_guess RO_KEF (<:RCCA(MS_KEM, A(RO_KEF)).O)).
+              by apply RCCA_lossless_dec.
+              by apply lossless_extract.
+          call{2} (_:true ==> true).
+            apply (lossless_guess RCCA1.O1 RCCA1.O2).
+              by apply RCCA1_lossless_dec.
+              by fun; sp; if => //; rnd; skip; smt.
 
-  fun main() : bool = {
-    var b, b' : bool;
-    var k0, k1 : ms;
-    var pk : pkey;
+      wp; rnd; wp; if{1}.
+        by rnd; skip; progress; smt.
+        by rnd{2}; skip; smt.
+  qed.
+  
+  local lemma Pr_RCCA1_res : forall &m, 
+    Pr[RCCA1.main() @ &m : res] <= 1%r / 2%r.
+  proof.
+    intros &m; bdhoare_deno (_:true) => //. 
+    fun; rnd; simplify; call (_:true) => //.  
+    wp; rnd; rnd; wp; call (_:true) => //.
+    inline V.init; call (_:true); wp; call (_:true); wp; call (_:true).
+    by skip; progress; try rewrite Bool.Dbool.mu_def; smt.
+  qed.
+  
+  local lemma Pr_RCCA_RCCA1 : forall &m,
+    Pr[RCCA(KEM(RO_KEF, PMS_KEM), A(RO_KEF)).main() @ &m : res] <=
+    1%r / 2%r + Pr[RCCA1.main() @ &m : RCCA1.abort].
+  proof.
+   intros &m.
+   apply (Trans _ (Pr[RCCA1.main() @ &m : res \/ RCCA1.abort])).
+     by equiv_deno RCCA_RCCA1; smt.  
+     by rewrite Pr mu_or; smt.
+  qed.
+  
+  
+  (** RCCA1 -> RCCA2 **)
+  
+  op find_ext sk (d:(label, (ms * version * hash * ciphertext)) map) h pms t = 
+   in_dom t d /\ 
+   let (k, pv, h', c) = proj d.[t] in h = h' /\ decrypt sk pv c = pms.
+  
+  local module RCCA2 = {
+    var m : (hash * (pms * label), ms) map
+    var d : (label, (ms * version * hash * ciphertext)) map
+   
+    module O1 = {
+      fun extract(p:hash, s:pms * label) : ms = {
+        var k : ms;
+        var pms : pms;
+        var t : label;
+        (pms, t) = s;
+        if (!in_dom (p, (pms, t)) m) {
+          if (find_ext V.sk d p pms t) {
+            k = let (ms, pv, h, c) = proj d.[t] in ms;
+          }
+          else k = $key;
+          m.[(p, (pms, t))] = k;
+        }
+        else k = proj m.[(p, (pms, t))];
+        return k;
+      }
+    }
+   
+    module O2 = {
+      fun dec(p:version * hash, t:label, c:ciphertext) : ms option = {
+        var pv : version;
+        var h : hash;
+        var k : ms;
+        var maybe_k : ms option = None;
+        if (!mem t V.labels /\ mem p P) { 
+          V.labels = add t V.labels;
+          (pv, h) = p;
+          if (!(V.guess /\ (pv, h) = pp /\ t = V.t /\ V.c = c)) {
+            if (in_dom (h, (decrypt V.sk pv c, t)) m) {
+              k = proj m.[(h, (decrypt V.sk pv c, t))];
+            }
+            else k = $key;
+            d.[t] = (k, pv, h, c);
+            maybe_k = if (!mem k V.keys) then Some k else None;
+          }
+        }
+        return maybe_k;
+      }
+    }
+    
+    module A = A(O1, O2)
+   
+    fun main() : bool = {
+      var b, b' : bool;
+      var k0, k1 : ms;
+      var pk : pkey;
+      PMS_KEM.init();
+      (pk, V.sk) = PMS_KEM.keygen();
+      V.init();
+      m = Core.empty;
+      d = Core.empty;
+      (V.pms, V.c) = PMS_KEM.enc((), pk, fst pp);
+      V.t = A.choose(pk);
+      k0 = $key;
+      k1 = $key;
+      V.guess = true;
+      V.keys = add k0 (add k1 V.keys);
+      b' = A.guess(V.c, k0);
+      return true;
+    }
+  }.
+  
+  local equiv RCCA1_RCCA2_extract : 
+    RCCA1.O1.extract ~ RCCA2.O1.extract :
+    ={p, s} /\ 
+    ={glob V} /\
+    (V.guess{1} => ={V.t}) /\
+    (decrypt V.sk (fst pp) V.c = V.pms){2} /\ 
+    (RCCA1.abort{1} =>
+     (exists t, in_dom (snd pp, (V.pms, t)) RCCA2.m \/
+     (V.guess /\ in_dom V.t RCCA2.d /\
+      let (k, pv, h, c) = proj RCCA2.d.[V.t] in
+       c <> V.c /\ decrypt V.sk pv c = V.pms)){2}) /\
+    (forall t, in_dom t RCCA2.d => mem t V.labels){2} /\
+    (forall h pms t, 
+     (in_dom (h, (pms, t)) RCCA1.m{1} <=>
+     (in_dom (h, (pms, t)) RCCA2.m{2} \/
+      (in_dom t RCCA2.d{2} /\ 
+       let (k, pv, h', c) = proj RCCA2.d{2}.[t] in 
+        h = h' /\ decrypt V.sk{2} pv c = pms)))) /\
+    (forall h pms t, 
+     (in_dom (h, (pms, t)) RCCA1.m{1} => 
+      in_dom (h, (pms, t)) RCCA2.m{2} => 
+      RCCA1.m{1}.[(h, (pms, t))] = RCCA2.m{2}.[(h, (pms, t))])) /\
+    (forall h pms t, 
+     (in_dom (h, (pms, t)) RCCA1.m{1} => 
+      !in_dom (h, (pms, t)) RCCA2.m{2} => 
+        RCCA1.m{1}.[(h, (pms, t))] = 
+        let (k, pv, h', c) = proj RCCA2.d{2}.[t] in Some k))
+    ==>
+    ={res} /\
+    ={glob V} /\
+    (V.guess{1} => ={V.t}) /\
+    (decrypt V.sk (fst pp) V.c = V.pms){2} /\ 
+    (RCCA1.abort{1} =>
+     (exists t, in_dom (snd pp, (V.pms, t)) RCCA2.m \/
+     (V.guess /\ in_dom V.t RCCA2.d /\
+      let (k, pv, h, c) = proj RCCA2.d.[V.t] in
+       c <> V.c /\ decrypt V.sk pv c = V.pms)){2}) /\
+    (forall t, in_dom t RCCA2.d => mem t V.labels){2} /\
+    (forall h pms t, 
+     (in_dom (h, (pms, t)) RCCA1.m{1} <=>
+     (in_dom (h, (pms, t)) RCCA2.m{2} \/
+      (in_dom t RCCA2.d{2} /\ 
+       let (k, pv, h', c) = proj RCCA2.d{2}.[t] in 
+        h = h' /\ decrypt V.sk{2} pv c = pms)))) /\
+    (forall h pms t, 
+     (in_dom (h, (pms, t)) RCCA1.m{1} => 
+      in_dom (h, (pms, t)) RCCA2.m{2} => 
+      RCCA1.m{1}.[(h, (pms, t))] = RCCA2.m{2}.[(h, (pms, t))])) /\
+    (forall h pms t, 
+     (in_dom (h, (pms, t)) RCCA1.m{1} => 
+      !in_dom (h, (pms, t)) RCCA2.m{2} => 
+        RCCA1.m{1}.[(h, (pms, t))] = 
+        let (k, pv, h', c) = proj RCCA2.d{2}.[t] in Some k)).
+  proof.
+    fun.
+    sp; if{1}.
+      rcondt{2} 1; first by intros &1; skip; intros &2; progress; smt.
+      sp; rcondf{2} 1.
+        intros &1; skip; intros &2; progress.
+        rewrite /find_ext; cut W := H1 p{2} pms{2} t{2}; smt.   
+      wp; rnd; skip; progress.
+        by smt.   
+        elim H8; clear H8; intros ?.
+          cut W : abortL = true by smt; subst.
+          by elim H; intros ? ?; exists t0; smt.       
+        by exists t{2}; smt.   
+        cut W := H1 h pms0 t0. 
+        case (in_dom (h, (pms0, t0)) RCCA1.m{1}); first by smt.
+        by intros ?; left; smt.
+        elim H8; clear H8; intros ?.
+          by case (in_dom (h, (pms0, t0)) RCCA2.m{2}); smt.
+          cut W := H1 h pms0 t0.
+          cut V : in_dom (h, (pms0, t0)) RCCA1.m{1}.
+          by elim W; intros _ X; apply X; smt.
+        by smt.
+        by cut W := H2 h pms0 t0; smt.    
+        by cut W := H1 h pms0 t0; cut X := H3 h pms0 t0; smt.
+       
+     if{2}.
+       sp; rcondt{2} 1.
+         by intros &1; skip; intros &2; progress; smt.
+       wp; skip; progress.
+         by smt.
+         elim H6; clear H6; intros ?.
+           cut W : abortL = true by smt; subst.
+           by elim H; intros ? ?; exists t0; smt.       
+         by exists t{2}; smt.
+         by cut W := H1 h pms0 t0; smt. 
+         elim H6; clear H6; intros ?.
+         case (in_dom (h, (pms0, t0)) RCCA2.m{2}); first by smt.
+         by intros ?; cut V : (h, (pms0, t0)) = (p, (pms, t)){2}; smt.
+         cut W := H1 h pms0 t0.
+         by elim W; intros _ X; apply X; smt.
+         by smt.
+         by smt.
+      by wp; skip; smt.
+  qed.
+  
+  local equiv RCCA1_RCCA2_dec :
+    RCCA1.O2.dec ~ RCCA2.O2.dec : 
+    ={p, t, c} /\ 
+    ={glob V} /\
+    (V.guess{1} => ={V.t}) /\
+    (decrypt V.sk (fst pp) V.c = V.pms){2} /\ 
+    (RCCA1.abort{1} =>
+     (exists t, in_dom (snd pp, (V.pms, t)) RCCA2.m \/
+     (V.guess /\ in_dom V.t RCCA2.d /\
+      let (k, pv, h, c) = proj RCCA2.d.[V.t] in
+       c <> V.c /\ decrypt V.sk pv c = V.pms)){2}) /\
+    (forall t, in_dom t RCCA2.d => mem t V.labels){2} /\
+    (forall h pms t, 
+     (in_dom (h, (pms, t)) RCCA1.m{1} <=>
+     (in_dom (h, (pms, t)) RCCA2.m{2} \/
+      (in_dom t RCCA2.d{2} /\ 
+       let (k, pv, h', c) = proj RCCA2.d{2}.[t] in 
+        h = h' /\ decrypt V.sk{2} pv c = pms)))) /\
+    (forall h pms t, 
+     (in_dom (h, (pms, t)) RCCA1.m{1} => 
+      in_dom (h, (pms, t)) RCCA2.m{2} => 
+      RCCA1.m{1}.[(h, (pms, t))] = RCCA2.m{2}.[(h, (pms, t))])) /\
+    (forall h pms t, 
+     (in_dom (h, (pms, t)) RCCA1.m{1} => 
+      !in_dom (h, (pms, t)) RCCA2.m{2} => 
+        RCCA1.m{1}.[(h, (pms, t))] = 
+        let (k, pv, h', c) = proj RCCA2.d{2}.[t] in Some k))
+    ==>
+    ={res} /\
+    ={glob V} /\
+    (V.guess{1} => ={V.t}) /\
+    (decrypt V.sk (fst pp) V.c = V.pms){2} /\ 
+    (RCCA1.abort{1} =>
+     (exists t, in_dom (snd pp, (V.pms, t)) RCCA2.m \/
+     (V.guess /\ in_dom V.t RCCA2.d /\
+      let (k, pv, h, c) = proj RCCA2.d.[V.t] in
+       c <> V.c /\ decrypt V.sk pv c = V.pms)){2}) /\
+    (forall t, in_dom t RCCA2.d => mem t V.labels){2} /\
+    (forall h pms t, 
+     (in_dom (h, (pms, t)) RCCA1.m{1} <=>
+     (in_dom (h, (pms, t)) RCCA2.m{2} \/
+      (in_dom t RCCA2.d{2} /\ 
+       let (k, pv, h', c) = proj RCCA2.d{2}.[t] in 
+        h = h' /\ decrypt V.sk{2} pv c = pms)))) /\
+    (forall h pms t, 
+     (in_dom (h, (pms, t)) RCCA1.m{1} => 
+      in_dom (h, (pms, t)) RCCA2.m{2} => 
+      RCCA1.m{1}.[(h, (pms, t))] = RCCA2.m{2}.[(h, (pms, t))])) /\
+    (forall h pms t, 
+     (in_dom (h, (pms, t)) RCCA1.m{1} => 
+      !in_dom (h, (pms, t)) RCCA2.m{2} => 
+        RCCA1.m{1}.[(h, (pms, t))] = 
+        let (k, pv, h', c) = proj RCCA2.d{2}.[t] in Some k)).
+  proof.
+     fun.
+     wp; sp; if => //.
+     inline{1} RCCA1.O1.extract.
+     seq 3 2 :
+      ((pms = decrypt V.sk pv c){1} /\
+       (pv{2}, h{2}) = p{2} /\
+       mem t{1} V.labels{1} /\
+       mem p{1} P /\
+       !in_dom t{2} RCCA2.d{2} /\
+       (pv{1}, h{1}) = p{1} /\
+       maybe_k{1} = None /\
+       ={maybe_k, p, t, c, glob V} /\
+      (V.guess{1} => ={V.t}) /\
+      (decrypt V.sk (fst pp) V.c = V.pms){2} /\ 
+      (RCCA1.abort{1} =>
+       (exists t, in_dom (snd pp, (V.pms, t)) RCCA2.m \/
+       (V.guess /\ in_dom V.t RCCA2.d /\
+        let (k, pv, h, c) = proj RCCA2.d.[V.t] in
+         c <> V.c /\ decrypt V.sk pv c = V.pms)){2}) /\
+      (forall t, in_dom t RCCA2.d => mem t V.labels){2} /\
+      (forall h pms t, 
+       (in_dom (h, (pms, t)) RCCA1.m{1} <=>
+       (in_dom (h, (pms, t)) RCCA2.m{2} \/
+        (in_dom t RCCA2.d{2} /\ 
+         let (k, pv, h', c) = proj RCCA2.d{2}.[t] in 
+          h = h' /\ decrypt V.sk{2} pv c = pms)))) /\
+      (forall h pms t, 
+       (in_dom (h, (pms, t)) RCCA1.m{1} => 
+        in_dom (h, (pms, t)) RCCA2.m{2} => 
+        RCCA1.m{1}.[(h, (pms, t))] = RCCA2.m{2}.[(h, (pms, t))])) /\
+      (forall h pms t, 
+       (in_dom (h, (pms, t)) RCCA1.m{1} => 
+        !in_dom (h, (pms, t)) RCCA2.m{2} => 
+          RCCA1.m{1}.[(h, (pms, t))] = 
+          let (k, pv, h', c) = proj RCCA2.d{2}.[t] in Some k))).
+        sp; wp; exists * V.sk{1}, pv{1}, c{1} ; elim *; intros sk pv c.
+        by call{1} (dec_spec sk pv c); skip; progress; smt.
+    
+        sp; if => //; first by smt.
+        if{1}.
+          if{2}.
+            by exfalso; smt.
+            wp; rnd; skip; progress.
+              by smt.
+              elim H13; clear H13; intros ?.
+              cut X : abortL = true by smt; subst.
+              by elim H2; smt.
+              exists t{2}.
+              by right; smt.
+              by smt.
+              case (in_dom (h0, (pms0, t0)) RCCA1.m{1}); first by smt.
+              by intros ?; cut Z : 
+                (h0, (pms0, t0)) =
+                (h{2}, (decrypt V.sk{2} pv{2} c{2}, t{2})); smt.
+              elim H13; clear H13; intros ?; first by smt.
+              case (t0 = t{2}).
+                intros ?; subst; elim H13; clear H13; intros X Y.
+                by generalize Y; rewrite /_.[_] Core.get_setE; smt.
+                intros ?.
+                cut L : (in_dom (h0, (pms0, t0)) RCCA1.m{1}); last by smt.
+                rewrite H4.
+                cut L : (in_dom t0 RCCA2.d{2} /\
+                  let (k0, pv0, h', c0) = proj RCCA2.d{2}.[t0] in
+                    h0 = h' /\ decrypt V.sk{2} pv0 c0 = pms0).
+                split; first by smt.
+                by generalize H13; rewrite /_.[_] Core.get_setN; smt.
+              by smt.
+              by smt.
+              case ((h, (decrypt V.sk pv c, t)){2} = (h0, (pms0, t0))).
+                by smt.
+                by intros ?; generalize H11; rewrite /_.[_] Core.get_setN; smt.
+      
+        (* similarly *)
+        rcondt{2} 1; first by intros &1; skip; intros &2; progress; smt.
+        wp; skip; progress.
+          by smt.
+          elim H9; clear H9; intros ?.
+          cut X : abortL = true by smt; subst.
+          by elim H2; smt.
+          by exists t{2}; right; smt.         
+          by smt.
+          by smt.
+          elim H9; clear H9; first by smt.
+          case (t0 = t{2}); first by smt.
+            intros ? [? ?].
+            case ((h, (decrypt V.sk pv c, t)){2} = (h0, (pms0, t0))).
+              by smt.
+              intros ?; rewrite H4; right; split; first by smt.
+              by generalize H11; rewrite /_.[_] Core.get_setN; smt.
+          by smt.
+  qed.
+  
+  local equiv RCCA1_RCCA2 :
+    RCCA1.main ~ RCCA2.main : 
+    true ==>
+    RCCA1.abort{1} =>
+      (exists t, in_dom (snd pp, (V.pms, t)) RCCA2.m){2} \/
+      (in_dom V.t RCCA2.d /\
+       let (k, pv, h, c) = proj RCCA2.d.[V.t] in
+         c <> V.c /\ decrypt V.sk pv c = V.pms){2}.
+  proof.
+    fun.
+    rnd{1}.
+    call (_:
+     ={glob V} /\
+     (V.guess{1} => ={V.t}) /\
+     (decrypt V.sk (fst pp) V.c = V.pms){2} /\ 
+     (RCCA1.abort{1} =>
+      (exists t, in_dom (snd pp, (V.pms, t)) RCCA2.m \/
+      (V.guess /\ in_dom V.t RCCA2.d /\
+       let (k, pv, h, c) = proj RCCA2.d.[V.t] in
+        c <> V.c /\ decrypt V.sk pv c = V.pms)){2}) /\
+     (forall t, in_dom t RCCA2.d => mem t V.labels){2} /\
+     (forall h pms t, 
+      (in_dom (h, (pms, t)) RCCA1.m{1} <=>
+      (in_dom (h, (pms, t)) RCCA2.m{2} \/
+       (in_dom t RCCA2.d{2} /\ 
+        let (k, pv, h', c) = proj RCCA2.d{2}.[t] in 
+         h = h' /\ decrypt V.sk{2} pv c = pms)))) /\
+     (forall h pms t, 
+      (in_dom (h, (pms, t)) RCCA1.m{1} => 
+       in_dom (h, (pms, t)) RCCA2.m{2} => 
+       RCCA1.m{1}.[(h, (pms, t))] = RCCA2.m{2}.[(h, (pms, t))])) /\
+     (forall h pms t, 
+      (in_dom (h, (pms, t)) RCCA1.m{1} => 
+       !in_dom (h, (pms, t)) RCCA2.m{2} => 
+         RCCA1.m{1}.[(h, (pms, t))] = 
+         let (k, pv, h', c) = proj RCCA2.d{2}.[t] in Some k))).
+      by apply RCCA1_RCCA2_dec.
+      by apply RCCA1_RCCA2_extract.
+    wp; rnd; rnd; wp.
+    call (_:
+     ={glob V} /\
+     (V.guess{1} => ={V.t}) /\
+     (decrypt V.sk (fst pp) V.c = V.pms){2} /\ 
+     (RCCA1.abort{1} =>
+      (exists t, in_dom (snd pp, (V.pms, t)) RCCA2.m \/
+      (V.guess /\ in_dom V.t RCCA2.d /\
+       let (k, pv, h, c) = proj RCCA2.d.[V.t] in
+        c <> V.c /\ decrypt V.sk pv c = V.pms)){2}) /\
+     (forall t, in_dom t RCCA2.d => mem t V.labels){2} /\
+     (forall h pms t, 
+      (in_dom (h, (pms, t)) RCCA1.m{1} <=>
+      (in_dom (h, (pms, t)) RCCA2.m{2} \/
+       (in_dom t RCCA2.d{2} /\ 
+        let (k, pv, h', c) = proj RCCA2.d{2}.[t] in 
+         h = h' /\ decrypt V.sk{2} pv c = pms)))) /\
+     (forall h pms t, 
+      (in_dom (h, (pms, t)) RCCA1.m{1} => 
+       in_dom (h, (pms, t)) RCCA2.m{2} => 
+       RCCA1.m{1}.[(h, (pms, t))] = RCCA2.m{2}.[(h, (pms, t))])) /\
+     (forall h pms t, 
+      (in_dom (h, (pms, t)) RCCA1.m{1} => 
+       !in_dom (h, (pms, t)) RCCA2.m{2} => 
+         RCCA1.m{1}.[(h, (pms, t))] = 
+         let (k, pv, h', c) = proj RCCA2.d{2}.[t] in Some k))).
+      by apply RCCA1_RCCA2_dec.
+      by apply RCCA1_RCCA2_extract. 
+    seq 2 2 : (={pk, V.sk} /\ keypair(pk, V.sk){1}).
+      by call keygen_rel; call (_:true); skip.
+      exists * pk{1}, V.sk{1}; elim *; intros pk sk.
+      call (enc_spec_rel pk sk (fst pp)).
+      by inline V.init; wp; skip; progress; smt.
+  qed.
+  
+  local lemma Pr_RCCA1_RCCA2 : forall &m,
+    Pr[RCCA1.main() @ &m : RCCA1.abort] <=
+    Pr[RCCA2.main() @ &m : exists t, in_dom (snd pp, (V.pms, t)) RCCA2.m] +  
+    Pr[RCCA2.main() @ &m : let (k, pv, h, c) = proj RCCA2.d.[V.t] in
+       c <> V.c /\ decrypt V.sk pv c = V.pms].
+  proof.
+    intros &m.
+    apply (Trans _ 
+      Pr[RCCA2.main() @ &m : 
+       (exists t, in_dom (snd pp, (V.pms, t)) RCCA2.m) \/
+       let (k, pv, h, c) = proj RCCA2.d.[V.t] in
+         c <> V.c /\ decrypt V.sk pv c = V.pms]).
+      by equiv_deno RCCA1_RCCA2; smt.  
+      rewrite Pr mu_or.
+      cut X : forall (x y z), 0%r <= z => x <= y => x - z <= y by smt.
+    by apply X; [smt | apply Refl].
+  qed.
+  
+  
+  (** RCCA2 -> OW_PCA **)
+  local module Find(PCO:PCA.Oracle) = {
+    var m : (hash * (pms * label), ms) map
+    var d : (label, (ms * version * hash * ciphertext)) map
+  
+    (* Private procedures *)
+    fun find(pv:version, c:ciphertext, h:hash, t:label) : pms option = {
+      var h' : hash;
+      var s : pms * label;
+      var pms : pms;
+      var t' : label;
+      var found : bool;
+      var q : (hash * (pms * label)) set;
+      var maybe_pms : pms option = None;
+      q = dom(m);
+      while (q <> FSet.empty /\ maybe_pms = None) {
+        (h',  s) = pick q;
+        q = rm (h', s) q;
+        (pms, t') = s;
+        found = PCO.check((), pms, pv, c);
+        maybe_pms = if found /\ h = h' /\ t = t' then Some pms else None; 
+      }
+      return maybe_pms;
+    }
+  
+    fun find_any(pv:version, c:ciphertext) : pms option = {
+      var h' : hash;
+      var s : pms * label;
+      var pms : pms;
+      var t' : label;
+      var found : bool;
+      var q : (hash * (pms * label)) set;
+      var maybe_pms : pms option = None;
+      q = dom(m);
+      while (q <> FSet.empty /\ maybe_pms = None) {
+        (h',  s) = pick q;
+        q = rm (h', s) q;
+        (pms, t') = s;
+        found = PCO.check((), pms, pv, c);
+        maybe_pms = if found then Some pms else None; 
+      }
+      return maybe_pms;
+    }
+
+    module O1 = {
+      fun extract(p:hash, s:pms * label) : ms = {
+        var k : ms;
+        var pms : pms;
+        var t : label;
+        var pv : version;
+        var h : hash;
+        var c : ciphertext;
+        var found : bool;
+        (pms, t) = s;
+        if (!in_dom (p, (pms, t)) m) {
+          (k, pv, h, c) = proj d.[t];
+          found = PCO.check((), pms, pv, c);
+          if (in_dom t d /\ p = h /\ found) {
+            k = let (ms, pv, h, c) = proj d.[t] in ms;
+          }
+          else k = $key;
+          m.[(p, (pms, t))] = k;
+        }
+        else k = proj m.[(p, (pms, t))];
+        return k;
+      }
+    }
+    
+    module O2 = {
+      fun dec(p:version * hash, t:label, c:ciphertext) : ms option = {
+        var pv : version;
+        var h : hash;
+        var k : ms;
+        var maybe_pms : pms option;
+        var maybe_k : ms option = None;
+        if (!mem t V.labels /\ mem p P) { 
+          V.labels = add t V.labels;
+          (pv, h) = p;
+          if (!(V.guess /\ (pv, h) = pp /\ t = V.t /\ V.c = c)) {
+            maybe_pms = find(pv, c, h, t);
+            if (maybe_pms <> None) k = proj m.[(h, (proj maybe_pms, t))];
+            else k = $key;
+            d.[t] = (k, pv, h, c);
+            maybe_k = if (!mem k V.keys) then Some k else None;
+          }
+        }
+        return maybe_k;
+      }
+    }
+  }.
+ 
+  local module B(PCO:PCA.Oracle) = {  
+    module F = Find(PCO)
+    module A = A(Find(PCO).O1, Find(PCO).O2)
+   
+    fun choose(pk:pkey) : version = {
+      var t : label;
+      V.init();
+      Find.m = Core.empty;
+      Find.d = Core.empty;
+      V.t = A.choose(pk);
+      return (fst pp);
+    }
+  
+    fun guess(c:ciphertext) : pms = {
+      var maybe_pms : pms option;
+      var k0, k1 : ms;
+      var b' : bool;
+      V.c = c;
+      k0 = $key;
+      k1 = $key;
+      V.keys = add k0 (add k1 V.keys);
+      V.guess = true;
+      b' = A.guess(c, k0);
+      maybe_pms = F.find_any(fst pp, c);
+      return proj maybe_pms;
+    }
+  }.
+ 
+  local lemma check_spec : forall _k _t _c,
+    bd_hoare 
+    [ PCA.Wrap(PMS_KEM).check : 
+      k = _k /\ t = _t /\ c = _c ==>
+      res <=> _k = decrypt PCA.V.sk _t _c ] = 1%r.
+  proof.
+    progress; fun.
+    exists * PCA.V.sk; elim *; intros sk.
+    by call (dec_spec sk _t _c); skip; progress; smt.
+  qed.
+  
+  local lemma find_any_spec : forall _pv _c,
+    bd_hoare 
+    [ Find(PCA.Wrap(PMS_KEM)).find_any : 
+      pv = _pv /\ c = _c ==> 
+      let pms = decrypt PCA.V.sk _pv _c in
+       ((exists h t, in_dom (h, (pms, t)) Find.m) <=> res = Some pms) /\
+       (res <> None => res = Some pms)] = 1%r.
+  proof.
+    progress; fun; sp.
+    while  
+     (let pms = decrypt PCA.V.sk pv c in
+      (forall x, mem x q => in_dom x Find.m) /\
+      (forall x, 
+       in_dom x Find.m => !mem x q => maybe_pms = None => pms <> fst (snd x)) /\
+      (maybe_pms <> None =>
+       (exists h t, in_dom (h, (pms, t)) Find.m) /\ maybe_pms = Some pms))
+     (card q).
+       intros z; sp; wp. 
+       exists * pms, pv, c; elim *; intros pms pv c.
+       by call (check_spec pms pv c); skip; progress; smt. 
+     by wp; skip; progress; smt.
+  qed.
+  
+  local lemma find_spec : forall _pv _c _h _t,
+    bd_hoare 
+    [ Find(PCA.Wrap(PMS_KEM)).find : 
+      pv = _pv /\ c = _c /\ h = _h /\ t = _t ==> 
+      let pms = decrypt PCA.V.sk _pv _c in
+       (in_dom (_h, (pms, _t)) Find.m <=> res = Some pms) /\
+       (res <> None => res = Some pms) ] = 1%r.
+  proof.
+    progress; fun; sp.
+    while  
+     (let pms = decrypt PCA.V.sk pv c in
+      (forall x, mem x q => in_dom x Find.m) /\
+      (forall x, 
+       in_dom x Find.m => !mem x q => maybe_pms = None => 
+       x <> (h, (pms, t))) /\
+      (maybe_pms <> None => 
+       in_dom (h, (pms, t)) Find.m /\ 
+       maybe_pms = Some pms /\ h = h' /\  t = t'))
+     (card q).
+      intros z; sp; wp. 
+      exists * pms, pv, c; elim *; intros pms pv c.
+      by call (check_spec pms pv c); skip; progress; smt. 
+    by wp; skip; progress; smt.
+  qed.
+  
+  local equiv RCCA2_OW_extract : 
+    RCCA2.O1.extract ~ Find(PCA.Wrap(PMS_KEM)).O1.extract :
+    ={p, s} /\ ={V.keys, V.labels, V.guess, V.t, V.c} /\
+    V.sk{1} = PCA.V.sk{2} /\ 
+    RCCA2.m{1} = Find.m{2} /\ 
+    RCCA2.d{1} = Find.d{2} 
+    ==>
+    ={res} /\ ={V.keys, V.labels, V.guess, V.t, V.c} /\
+    V.sk{1} = PCA.V.sk{2} /\ 
+    RCCA2.m{1} = Find.m{2} /\ 
+    RCCA2.d{1} = Find.d{2}. 
+  proof.
+    fun.
+    sp; if => //.
+      seq 0 2 : 
+       (={pms, t, p, s, V.keys, V.labels, V.guess, V.t, V.c} /\
+        V.sk{1} = PCA.V.sk{2} /\ 
+        RCCA2.m{1} = Find.m{2} /\ 
+        RCCA2.d{1} = Find.d{2} /\
+        ((find_ext V.sk RCCA2.d p pms t){1} <=> 
+         (in_dom t Find.d /\ p = h /\ found){2})).
+        sp; exists * pms{2}, pv{2}, c{2}; elim *; intros pms pv c.
+        by call{2} (check_spec pms pv c); skip; progress; smt.
+        by if => //; wp; try rnd; skip; progress.
+      by wp.
+  qed.
+  
+  local equiv RCCA2_OW_dec : 
+    RCCA2.O2.dec ~ Find(PCA.Wrap(PMS_KEM)).O2.dec :
+    ={p, t, c} /\ ={V.keys, V.labels, V.guess, V.t, V.c} /\
+    V.sk{1} = PCA.V.sk{2} /\ 
+    RCCA2.m{1} = Find.m{2} /\ 
+    RCCA2.d{1} = Find.d{2} 
+    ==>
+    ={res} /\ ={V.keys, V.labels, V.guess, V.t, V.c} /\
+    V.sk{1} = PCA.V.sk{2} /\ 
+    RCCA2.m{1} = Find.m{2} /\ 
+    RCCA2.d{1} = Find.d{2}. 
+  proof.
+    fun.
+    sp; if => //.
+    sp; if => //.
+    seq 0 1 :    
+     (maybe_k{1} = None /\
+      ={maybe_k, pv, h, p, t, c, V.labels, V.keys, V.guess, V.t, V.c} /\
+      V.sk{1} = PCA.V.sk{2} /\
+      RCCA2.m{1} = Find.m{2} /\ 
+      RCCA2.d{1} = Find.d{2} /\
+      !(V.guess /\ (pv, h) = pp /\ t = V.t /\ V.c = c){1} /\
+      ((in_dom (h, (decrypt V.sk pv c, t)) RCCA2.m){1} <=> 
+       maybe_pms{2} <> None) /\
+      (maybe_pms <> None => 
+       maybe_pms = Some (decrypt PCA.V.sk pv c)){2}).
+      sp; exists * pv{2}, c{2}, h{2}, t{2}; elim *; intros pv c h t.
+      by call{2} (find_spec pv c h t); skip; progress; smt.  
+      if => //.
+        by wp; skip; smt.
+        by wp; rnd.
+  qed.
+  
+  local equiv RCCA2_OW :
+    RCCA2.main ~ PCA.OW_PCA(PMS_KEM, B).main :
+    true ==> (exists t, in_dom (snd pp, (V.pms, t)) RCCA2.m){1} => res{2}.
+  proof.
+   fun.
+   (* Workaround to swap PMS_KEM.enc *)
+   transitivity{1} {
     PMS_KEM.init();
     (pk, V.sk) = PMS_KEM.keygen();
     V.init();
-    m = Core.empty;
-    d = Core.empty;
-    (V.pms, V.c) = PMS_KEM.enc((), pk, fst p');
-    V.t = A.choose(pk);
-    k0 = $Outer_KEM.key;
-    k1 = $Outer_KEM.key;
+    RCCA2.m = Core.empty;
+    RCCA2.d = Core.empty;
+    V.t = RCCA2.A.choose(pk);
+    (V.pms, V.c) = PMS_KEM.enc((), pk, fst pp);
+    k0 = $key;
+    k1 = $key;
     V.guess = true;
     V.keys = add k0 (add k1 V.keys);
-    b' = A.guess(V.c, k0);
-    return true;
-  }
- }.
-
- local equiv RCCA1_RCCA2_extract : 
-   RCCA1.O.extract ~ RCCA2.O.extract :
-   ={p, s} /\ 
-   ={glob V} /\
-   (V.guess{1} => ={V.t}) /\
-   (decrypt () V.sk (fst p') V.c = V.pms){2} /\ 
-   (RCCA1.abort{1} =>
-    (exists t, in_dom (snd p', (V.pms, t)) RCCA2.m \/
-    (V.guess /\ in_dom V.t RCCA2.d /\
-     let (k, pv, h, c) = proj RCCA2.d.[V.t] in
-      c <> V.c /\ decrypt () V.sk pv c = V.pms)){2}) /\
-   (forall t, in_dom t RCCA2.d => mem t V.labels){2} /\
-   (forall h pms t, 
-    (in_dom (h, (pms, t)) RCCA1.m{1} <=>
-    (in_dom (h, (pms, t)) RCCA2.m{2} \/
-     (in_dom t RCCA2.d{2} /\ 
-      let (k, pv, h', c) = proj RCCA2.d{2}.[t] in 
-       h = h' /\ decrypt () V.sk{2} pv c = pms)))) /\
-   (forall h pms t, 
-    (in_dom (h, (pms, t)) RCCA1.m{1} => 
-     in_dom (h, (pms, t)) RCCA2.m{2} => 
-     RCCA1.m{1}.[(h, (pms, t))] = RCCA2.m{2}.[(h, (pms, t))])) /\
-   (forall h pms t, 
-    (in_dom (h, (pms, t)) RCCA1.m{1} => 
-     !in_dom (h, (pms, t)) RCCA2.m{2} => 
-       RCCA1.m{1}.[(h, (pms, t))] = 
-       let (k, pv, h', c) = proj RCCA2.d{2}.[t] in Some k))
-   ==>
-   ={res} /\
-   ={glob V} /\
-   (V.guess{1} => ={V.t}) /\
-   (decrypt () V.sk (fst p') V.c = V.pms){2} /\ 
-   (RCCA1.abort{1} =>
-    (exists t, in_dom (snd p', (V.pms, t)) RCCA2.m \/
-    (V.guess /\ in_dom V.t RCCA2.d /\
-     let (k, pv, h, c) = proj RCCA2.d.[V.t] in
-      c <> V.c /\ decrypt () V.sk pv c = V.pms)){2}) /\
-   (forall t, in_dom t RCCA2.d => mem t V.labels){2} /\
-   (forall h pms t, 
-    (in_dom (h, (pms, t)) RCCA1.m{1} <=>
-    (in_dom (h, (pms, t)) RCCA2.m{2} \/
-     (in_dom t RCCA2.d{2} /\ 
-      let (k, pv, h', c) = proj RCCA2.d{2}.[t] in 
-       h = h' /\ decrypt () V.sk{2} pv c = pms)))) /\
-   (forall h pms t, 
-    (in_dom (h, (pms, t)) RCCA1.m{1} => 
-     in_dom (h, (pms, t)) RCCA2.m{2} => 
-     RCCA1.m{1}.[(h, (pms, t))] = RCCA2.m{2}.[(h, (pms, t))])) /\
-   (forall h pms t, 
-    (in_dom (h, (pms, t)) RCCA1.m{1} => 
-     !in_dom (h, (pms, t)) RCCA2.m{2} => 
-       RCCA1.m{1}.[(h, (pms, t))] = 
-       let (k, pv, h', c) = proj RCCA2.d{2}.[t] in Some k)).
- proof.
-  fun.
-  sp; if{1}.
-   rcondt{2} 1; first by intros &1; skip; intros &2; progress; smt.
-   sp; rcondf{2} 1.
-    intros &1; skip; intros &2; progress.
-    rewrite /find_ext; cut W := H1 p{2} pms{2} t{2}; smt.
-
-   wp; rnd; skip; progress.
-    by smt.
-
-    elim H8; clear H8; intros ?.
-     cut W : abortL = true by smt; subst.
-     by elim H; intros ? ?; exists t0; smt.
-     
-     by exists t{2}; smt.
-
-    cut W := H1 h pms0 t0. 
-    case (in_dom (h, (pms0, t0)) RCCA1.m{1}); first by smt.
-     intros ?; left; smt.
-
-    elim H8; clear H8; intros ?.
-     by case (in_dom (h, (pms0, t0)) RCCA2.m{2}); smt.
-
-    cut W := H1 h pms0 t0; cut V : in_dom (h, (pms0, t0)) RCCA1.m{1}.
-     by elim W; intros _ X; apply X; smt.
-    by smt.
-    
-    by cut W := H2 h pms0 t0; smt.    
-    by cut W := H1 h pms0 t0; cut X := H3 h pms0 t0; smt.    
-
-   if{2}.
-    sp; rcondt{2} 1.
-     intros &1; skip; intros &2; progress; smt.
-
-    wp; skip; progress.
-     by smt.
-
-     elim H6; clear H6; intros ?.
-      cut W : abortL = true by smt; subst.
-      by elim H; intros ? ?; exists t0; smt.
-     
-      by exists t{2}; smt.
-
-    by cut W := H1 h pms0 t0; smt. 
-
-    elim H6; clear H6; intros ?.
-    case (in_dom (h, (pms0, t0)) RCCA2.m{2}); first by smt.
-    intros ?; cut V : (h, (pms0, t0)) = (p, (pms, t)){2}; smt.
-
-    cut W := H1 h pms0 t0.
-    by elim W; intros _ X; apply X; smt.
- 
-    by smt.
-    by smt.
-
-   by wp; skip; progress; smt.
- qed.
-
- local equiv RCCA1_RCCA2_dec :
-   RCCA1.O.dec ~ RCCA2.O.dec : 
-   ={p, t, c} /\ 
-   ={glob V} /\
-   (V.guess{1} => ={V.t}) /\
-   (decrypt () V.sk (fst p') V.c = V.pms){2} /\ 
-   (RCCA1.abort{1} =>
-    (exists t, in_dom (snd p', (V.pms, t)) RCCA2.m \/
-    (V.guess /\ in_dom V.t RCCA2.d /\
-     let (k, pv, h, c) = proj RCCA2.d.[V.t] in
-      c <> V.c /\ decrypt () V.sk pv c = V.pms)){2}) /\
-   (forall t, in_dom t RCCA2.d => mem t V.labels){2} /\
-   (forall h pms t, 
-    (in_dom (h, (pms, t)) RCCA1.m{1} <=>
-    (in_dom (h, (pms, t)) RCCA2.m{2} \/
-     (in_dom t RCCA2.d{2} /\ 
-      let (k, pv, h', c) = proj RCCA2.d{2}.[t] in 
-       h = h' /\ decrypt () V.sk{2} pv c = pms)))) /\
-   (forall h pms t, 
-    (in_dom (h, (pms, t)) RCCA1.m{1} => 
-     in_dom (h, (pms, t)) RCCA2.m{2} => 
-     RCCA1.m{1}.[(h, (pms, t))] = RCCA2.m{2}.[(h, (pms, t))])) /\
-   (forall h pms t, 
-    (in_dom (h, (pms, t)) RCCA1.m{1} => 
-     !in_dom (h, (pms, t)) RCCA2.m{2} => 
-       RCCA1.m{1}.[(h, (pms, t))] = 
-       let (k, pv, h', c) = proj RCCA2.d{2}.[t] in Some k))
-   ==>
-   ={res} /\
-   ={glob V} /\
-   (V.guess{1} => ={V.t}) /\
-   (decrypt () V.sk (fst p') V.c = V.pms){2} /\ 
-   (RCCA1.abort{1} =>
-    (exists t, in_dom (snd p', (V.pms, t)) RCCA2.m \/
-    (V.guess /\ in_dom V.t RCCA2.d /\
-     let (k, pv, h, c) = proj RCCA2.d.[V.t] in
-      c <> V.c /\ decrypt () V.sk pv c = V.pms)){2}) /\
-   (forall t, in_dom t RCCA2.d => mem t V.labels){2} /\
-   (forall h pms t, 
-    (in_dom (h, (pms, t)) RCCA1.m{1} <=>
-    (in_dom (h, (pms, t)) RCCA2.m{2} \/
-     (in_dom t RCCA2.d{2} /\ 
-      let (k, pv, h', c) = proj RCCA2.d{2}.[t] in 
-       h = h' /\ decrypt () V.sk{2} pv c = pms)))) /\
-   (forall h pms t, 
-    (in_dom (h, (pms, t)) RCCA1.m{1} => 
-     in_dom (h, (pms, t)) RCCA2.m{2} => 
-     RCCA1.m{1}.[(h, (pms, t))] = RCCA2.m{2}.[(h, (pms, t))])) /\
-   (forall h pms t, 
-    (in_dom (h, (pms, t)) RCCA1.m{1} => 
-     !in_dom (h, (pms, t)) RCCA2.m{2} => 
-       RCCA1.m{1}.[(h, (pms, t))] = 
-       let (k, pv, h', c) = proj RCCA2.d{2}.[t] in Some k)).
- proof.
-  fun.
-  wp; sp; if => //.
-  inline{1} RCCA1.O.extract.
-  seq 3 2 :
-   ((pms = decrypt () V.sk pv c){1} /\
-    (pv{2}, h{2}) = p{2} /\
-    mem t{1} V.labels{1} /\
-    mem p{1} P /\
-    !in_dom t{2} RCCA2.d{2} /\
-    (pv{1}, h{1}) = p{1} /\
-    maybe_k{1} = None /\
-    ={maybe_k, p, t, c, glob V} /\
-   (V.guess{1} => ={V.t}) /\
-   (decrypt () V.sk (fst p') V.c = V.pms){2} /\ 
-   (RCCA1.abort{1} =>
-    (exists t, in_dom (snd p', (V.pms, t)) RCCA2.m \/
-    (V.guess /\ in_dom V.t RCCA2.d /\
-     let (k, pv, h, c) = proj RCCA2.d.[V.t] in
-      c <> V.c /\ decrypt () V.sk pv c = V.pms)){2}) /\
-   (forall t, in_dom t RCCA2.d => mem t V.labels){2} /\
-   (forall h pms t, 
-    (in_dom (h, (pms, t)) RCCA1.m{1} <=>
-    (in_dom (h, (pms, t)) RCCA2.m{2} \/
-     (in_dom t RCCA2.d{2} /\ 
-      let (k, pv, h', c) = proj RCCA2.d{2}.[t] in 
-       h = h' /\ decrypt () V.sk{2} pv c = pms)))) /\
-   (forall h pms t, 
-    (in_dom (h, (pms, t)) RCCA1.m{1} => 
-     in_dom (h, (pms, t)) RCCA2.m{2} => 
-     RCCA1.m{1}.[(h, (pms, t))] = RCCA2.m{2}.[(h, (pms, t))])) /\
-   (forall h pms t, 
-    (in_dom (h, (pms, t)) RCCA1.m{1} => 
-     !in_dom (h, (pms, t)) RCCA2.m{2} => 
-       RCCA1.m{1}.[(h, (pms, t))] = 
-       let (k, pv, h', c) = proj RCCA2.d{2}.[t] in Some k))).
-   sp; wp; exists * V.sk{1}, pv{1}, c{1} ; elim *; intros sk pv c.
-   by call{1} (dec_spec sk pv c); skip; progress; smt.
- 
-   sp; if => //; first by smt.
-   if{1}.
-    if{2}.
-     by exfalso; progress; rewrite /find_dec; smt.
-     wp; rnd; skip; progress.
-      by smt.
- 
-      elim H13; clear H13; intros ?.
-       cut X : abortL = true by smt; subst.
-       by elim H2; smt.
+    b' = RCCA2.A.guess(V.c, k0);
+   }
+   (true ==> ={glob V, RCCA2.m, RCCA2.d})
+   (true ==> (exists t, in_dom (snd pp, (V.pms, t)) RCCA2.m){1} => (k = k'){2}) => //.
+   call (_: ={glob V, RCCA2.m, RCCA2.d}).
+    by fun; eqobs_in.
+    by fun; eqobs_in.
+    wp; rnd; rnd; simplify.
+    seq 5 5 : (={glob V, pk, RCCA2.m, RCCA2.d}); first by eqobs_in.
+    seq 2 2 : (={glob A, glob V, pk, RCCA2.m, RCCA2.d}).
+      admit (* swap, but technically dec 'uses' V.c *).
+      by trivial.
+   (*********************************)
+   inline PCA.OW_PCA(PMS_KEM, B).A.choose 
+          PCA.OW_PCA(PMS_KEM, B).A.guess.
+   wp; seq 6 7 : (={pk, glob A, V.keys, V.labels, V.guess, V.t, V.c} /\
+    keypair(pk, V.sk){1} /\
+    V.sk{1} = PCA.V.sk{2} /\ 
+    RCCA2.m{1} = Find.m{2} /\ 
+    RCCA2.d{1} = Find.d{2}).
+      call (_: ={V.keys, V.labels, V.guess, V.t, V.c} /\
+        V.sk{1} = PCA.V.sk{2} /\ 
+        RCCA2.m{1} = Find.m{2} /\ RCCA2.d{1} = Find.d{2}).
+        by apply RCCA2_OW_dec.
+        by apply RCCA2_OW_extract.
+      inline V.init; wp; call keygen_rel; wp; call (_:true); skip; smt.
+    seq 1 2 :
+     (={pk, glob A, V.keys, V.labels, V.guess, V.t} /\
+      (decrypt V.sk (fst pp) V.c = V.pms){1} /\
+      V.pms{1} = k{2} /\ V.c{1} = c{2} /\
+      V.sk{1} = PCA.V.sk{2} /\ 
+      RCCA2.m{1} = Find.m{2} /\ RCCA2.d{1} = Find.d{2}).
+      exists * V.sk{1}, pk{1}; elim *; intros sk pk.
+      by call (enc_spec_rel pk sk (fst pp)); wp; skip; smt.  
+    seq 5 7 : (={pk, glob A, V.keys, V.labels, V.guess, V.t, V.c} /\ 
+     V.sk{1} = PCA.V.sk{2} /\ 
+     V.pms{1} = k{2} /\
+     (decrypt V.sk (fst pp) V.c = V.pms){1} /\
+     V.pms{1} = k{2} /\ V.c{1} = c0{2} /\
+     RCCA2.m{1} = Find.m{2} /\ RCCA2.d{1} = Find.d{2}).
+     call (_: ={V.keys, V.labels, V.guess, V.t, V.c} /\
+      V.sk{1} = PCA.V.sk{2} /\ 
+      RCCA2.m{1} = Find.m{2} /\ 
+      RCCA2.d{1} = Find.d{2}).
+       by apply RCCA2_OW_dec.
+       by apply RCCA2_OW_extract.
+     by wp; rnd; rnd; wp.  
+    exists * c0{2}; elim *; intros c.
+    call{2} (find_any_spec (fst pp) c).
+    by wp; skip; progress; smt.
+  qed.
+  
+  local lemma Pr_RCCA2_OW : forall &m,
+    Pr[RCCA2.main() @ &m : exists t, in_dom (snd pp, (V.pms, t)) RCCA2.m] <=
+    Pr[PCA.OW_PCA(PMS_KEM, B).main() @ &m : res].
+  proof.
+    by intros &m; equiv_deno RCCA2_OW.
+  qed.
+  
+  
+  (** RCCA2 -> NR *)
+  
+  local module C(PCO:PCA.Oracle) = {
+    module F = Find(PCO)
+    module A = A(Find(PCO).O1, Find(PCO).O2)
       
-       exists t{2}.
-       by generalize H9; rewrite /find_dec; intros ?; right; smt.
-     
-      by smt.
-
-     case (in_dom (h0, (pms0, t0)) RCCA1.m{1}); first by smt.
-     intros ?;
-     cut Z : 
-       (h0, (pms0, t0)) =
-       (h{2}, (decrypt () V.sk{2} pv{2} c{2}, t{2})) by smt.
-     by smt.
-
-     elim H13; clear H13; intros ?; first by smt.
-     case (t0 = t{2}).
-      intros ?; subst; elim H13; clear H13; intros X Y.
-      by generalize Y; rewrite /_.[_] Core.get_setE; smt.
-      intros ?; cut L : (in_dom (h0, (pms0, t0)) RCCA1.m{1}); last by smt.
-      rewrite H4.
-      cut L : (in_dom t0 RCCA2.d{2} /\
-        let (k0, pv0, h', c0) = proj RCCA2.d{2}.[t0] in
-        h0 = h' /\ decrypt () V.sk{2} pv0 c0 = pms0).
-      split; first by smt.
-      by generalize H13; rewrite /_.[_] Core.get_setN; smt.
-     
-      by smt.
-   
-     by smt.
-     by case ((h, (decrypt () V.sk pv c, t)){2} = (h0, (pms0, t0))); smt.
-   
-   (* the same *)
-   rcondt{2} 1; first by intros &1; skip; intros &2; progress; smt.
-   wp; skip; progress.
-    by smt.
-  
-    elim H9; clear H9; intros ?.
-     cut X : abortL = true by smt; subst.
-     by elim H2; smt.
-
-     exists t{2}.
-     by generalize H9; rewrite /find_dec; intros ?; right; smt.
-    
-    by smt.
-    by smt.
-
-    elim H9; clear H9; first by smt.
-    case (t0 = t{2}); first by smt.
-    intros ? [? ?].
-    case ((h, (decrypt () V.sk pv c, t)){2} = (h0, (pms0, t0))); first by smt.
-    intros ?; rewrite H4; right; split; first by smt.
-    by generalize H11; rewrite /_.[_] Core.get_setN; smt.
-
-   by smt.
- qed.
-
- local equiv RCCA1_RCCA2 :
-   RCCA1.main ~ RCCA2.main : 
-   true ==>
-   RCCA1.abort{1} =>
-    (exists t, in_dom (snd p', (V.pms, t)) RCCA2.m){2} \/
-    (in_dom V.t RCCA2.d /\
-     let (k, pv, h, c) = proj RCCA2.d.[V.t] in
-      c <> V.c /\ decrypt () V.sk pv c = V.pms){2}.
- proof.
-  fun.
-  rnd{1}.
-  call (_:
-   ={glob V} /\
-   (V.guess{1} => ={V.t}) /\
-   (decrypt () V.sk (fst p') V.c = V.pms){2} /\ 
-   (RCCA1.abort{1} =>
-    (exists t, in_dom (snd p', (V.pms, t)) RCCA2.m \/
-    (V.guess /\ in_dom V.t RCCA2.d /\
-     let (k, pv, h, c) = proj RCCA2.d.[V.t] in
-      c <> V.c /\ decrypt () V.sk pv c = V.pms)){2}) /\
-   (forall t, in_dom t RCCA2.d => mem t V.labels){2} /\
-   (forall h pms t, 
-    (in_dom (h, (pms, t)) RCCA1.m{1} <=>
-    (in_dom (h, (pms, t)) RCCA2.m{2} \/
-     (in_dom t RCCA2.d{2} /\ 
-      let (k, pv, h', c) = proj RCCA2.d{2}.[t] in 
-       h = h' /\ decrypt () V.sk{2} pv c = pms)))) /\
-   (forall h pms t, 
-    (in_dom (h, (pms, t)) RCCA1.m{1} => 
-     in_dom (h, (pms, t)) RCCA2.m{2} => 
-     RCCA1.m{1}.[(h, (pms, t))] = RCCA2.m{2}.[(h, (pms, t))])) /\
-   (forall h pms t, 
-    (in_dom (h, (pms, t)) RCCA1.m{1} => 
-     !in_dom (h, (pms, t)) RCCA2.m{2} => 
-       RCCA1.m{1}.[(h, (pms, t))] = 
-       let (k, pv, h', c) = proj RCCA2.d{2}.[t] in Some k))).
-   by apply RCCA1_RCCA2_dec.
-   by apply RCCA1_RCCA2_extract.
-  wp; rnd; rnd; wp.
-  call (_:
-   ={glob V} /\
-   (V.guess{1} => ={V.t}) /\
-   (decrypt () V.sk (fst p') V.c = V.pms){2} /\ 
-   (RCCA1.abort{1} =>
-    (exists t, in_dom (snd p', (V.pms, t)) RCCA2.m \/
-    (V.guess /\ in_dom V.t RCCA2.d /\
-     let (k, pv, h, c) = proj RCCA2.d.[V.t] in
-      c <> V.c /\ decrypt () V.sk pv c = V.pms)){2}) /\
-   (forall t, in_dom t RCCA2.d => mem t V.labels){2} /\
-   (forall h pms t, 
-    (in_dom (h, (pms, t)) RCCA1.m{1} <=>
-    (in_dom (h, (pms, t)) RCCA2.m{2} \/
-     (in_dom t RCCA2.d{2} /\ 
-      let (k, pv, h', c) = proj RCCA2.d{2}.[t] in 
-       h = h' /\ decrypt () V.sk{2} pv c = pms)))) /\
-   (forall h pms t, 
-    (in_dom (h, (pms, t)) RCCA1.m{1} => 
-     in_dom (h, (pms, t)) RCCA2.m{2} => 
-     RCCA1.m{1}.[(h, (pms, t))] = RCCA2.m{2}.[(h, (pms, t))])) /\
-   (forall h pms t, 
-    (in_dom (h, (pms, t)) RCCA1.m{1} => 
-     !in_dom (h, (pms, t)) RCCA2.m{2} => 
-       RCCA1.m{1}.[(h, (pms, t))] = 
-       let (k, pv, h', c) = proj RCCA2.d{2}.[t] in Some k))).
-   by apply RCCA1_RCCA2_dec.
-   by apply RCCA1_RCCA2_extract. 
-  seq 2 2 : (={pk, V.sk}); first by eqobs_in.
-  exists * pk{1}, V.sk{1}; elim *; intros pk sk.
-  call (enc_spec_rel pk sk (fst p')).
-  by inline V.init; wp; skip; progress; smt.
- qed.
-
- local lemma Pr_RCCA1_RCCA2 : forall &m,
-   Pr[RCCA1.main() @ &m : RCCA1.abort] <=
-   Pr[RCCA2.main() @ &m : exists t, in_dom (snd p', (V.pms, t)) RCCA2.m] +  
-   Pr[RCCA2.main() @ &m : let (k, pv, h, c) = proj RCCA2.d.[V.t] in
-      c <> V.c /\ decrypt () V.sk pv c = V.pms].
- proof.
-  intros &m.
-  apply (Trans _ 
-   Pr[RCCA2.main() @ &m : 
-    (exists t, in_dom (snd p', (V.pms, t)) RCCA2.m) \/
-    let (k, pv, h, c) = proj RCCA2.d.[V.t] in
-     c <> V.c /\ decrypt () V.sk pv c = V.pms]).
-  equiv_deno RCCA1_RCCA2; smt.  
-  rewrite Pr mu_or.
-  cut X : forall (x y z:real), 0%r <= z => x <= y => x - z <= y by smt.
-  by apply X; [smt | apply Refl].
- qed.
-
-
- (** RCCA2 -> OW_PCA **)
-
- local module B(PCO:OW_PCA.Oracles) = {
-  var m : (hash * (pms * label), ms) map
-  var d : (label, (ms * version * hash * ciphertext)) map
-
-  (* Private procedures *)
-  fun find(pv:version, c:ciphertext, h:hash, t:label) : pms option = {
-    var h' : hash;
-    var s : pms * label;
-    var pms : pms;
-    var t' : label;
-    var found : bool;
-    var q : (hash * (pms * label)) set;
-    var maybe_pms : pms option = None;
-    q = dom(m);
-    while (q <> FSet.empty /\ maybe_pms = None) {
-      (h',  s) = pick q;
-      q = rm (h', s) q;
-      (pms, t') = s;
-      found = PCO.check((), pms, pv, c);
-      maybe_pms = if found /\ h = h' /\ t = t' then Some pms else None; 
+    fun choose(pk:pkey) : version = {
+      var t : label;
+      V.init();
+      Find.m = Core.empty;
+      Find.d = Core.empty;
+      V.t = A.choose(pk);
+      return (fst pp);
     }
-    return maybe_pms;
-  }
-
-  fun find_any(pv:version, c:ciphertext) : pms option = {
-    var h' : hash;
-    var s : pms * label;
-    var pms : pms;
-    var t' : label;
-    var found : bool;
-    var q : (hash * (pms * label)) set;
-    var maybe_pms : pms option = None;
-    q = dom(m);
-    while (q <> FSet.empty /\ maybe_pms = None) {
-      (h',  s) = pick q;
-      q = rm (h', s) q;
-      (pms, t') = s;
-      found = PCO.check((), pms, pv, c);
-      maybe_pms = if found then Some pms else None; 
+  
+    fun guess(c:ciphertext) : version * ciphertext = {
+      var pms : pms;
+      var k0, k1 : ms;
+      var b' : bool;
+      V.c = c;
+      k0 = $key;
+      k1 = $key;
+      V.keys = add k0 (add k1 V.keys);
+      V.guess = true;
+      b' = A.guess(c, k0);
+      return let (k, pv, h, c) = proj Find.d.[V.t] in (pv, c);
     }
-    return maybe_pms;
-  }
-
-  module O = {
-   fun extract(p:hash, s:pms * label) : ms = {
-     var k : ms;
-     var pms : pms;
-     var t : label;
-     var pv : version;
-     var h : hash;
-     var c : ciphertext;
-     var found : bool;
-     (pms, t) = s;
-     if (!in_dom (p, (pms, t)) m) {
-       (k, pv, h, c) = proj d.[t];
-       found = PCO.check((), pms, pv, c);
-       if (in_dom t d /\ p = h /\ found) {
-         k = let (ms, pv, h, c) = proj d.[t] in ms;
-       }
-       else k = $Outer_KEM.key;
-       m.[(p, (pms, t))] = k;
-     }
-     else {
-       k = proj m.[(p, (pms, t))];
-     }
-     return k;
-   }
-
-   fun dec(p:version * hash, t:label, c:ciphertext) : ms option = {
-     var pv : version;
-     var h : hash;
-     var k : ms;
-     var maybe_pms : pms option;
-     var maybe_k : ms option = None;
-     if (!mem t V.labels /\ mem p P) { 
-       V.labels = add t V.labels;
-       (pv, h) = p;
-       if (!(V.guess /\ (pv, h) = p' /\ t = V.t /\ V.c = c)) {
-         maybe_pms = find(pv, c, h, t);
-         if (maybe_pms <> None) {
-           k = proj m.[(h, (proj maybe_pms, t))];
-         }
-         else {
-           k = $Outer_KEM.key;
-         }
-         d.[t] = (k, pv, h, c);
-         maybe_k = if (!mem k V.keys) then Some k else None;
-       }
-     }
-     return maybe_k;
-   }
-  }
+  }.
   
-  module A = A(O, O)
-  
-  fun choose(pk:pkey) : version = {
-    var t : label;
-    V.init();
-    m = Core.empty;
-    d = Core.empty;
-    V.t = A.choose(pk);
-    return (fst p');
-  }
-
-  fun guess(c:ciphertext) : pms = {
-    var maybe_pms : pms option;
-    var k0, k1 : ms;
-    var b' : bool;
-    V.c = c;
-    k0 = $Outer_KEM.key;
-    k1 = $Outer_KEM.key;
-    V.keys = add k0 (add k1 V.keys);
-    V.guess = true;
-    b' = A.guess(c, k0);
-    maybe_pms = find_any(fst p', c);
-    return proj maybe_pms;
-  }
- }.
-
- local lemma check_spec : forall _p _k _t _c,
-   bd_hoare 
-   [ OW_PCA.OW_PCA(PMS_KEM, B).O.check : 
-     p = _p /\ k = _k /\ t = _t /\ c = _c ==>
-    res <=> _k = decrypt _p OW_PCA.OW_PCA.sk _t _c ] = 1%r.
- proof.
-  progress; fun.
-  exists * OW_PCA.OW_PCA.sk; elim *; intros sk.
-  by call (dec_spec sk _t _c); skip; progress; smt.
- qed.
-
- local lemma find_any_spec : forall (_pv:version) (_c:ciphertext),
-   bd_hoare 
-   [ B(OW_PCA.OW_PCA(PMS_KEM, B).O).find_any : 
-     pv = _pv /\ c = _c ==> 
-     let pms = decrypt () OW_PCA.OW_PCA.sk _pv _c in
-      ((exists h t, in_dom (h, (pms, t)) B.m) <=> res = Some pms) /\
-      (res <> None => res = Some pms)] = 1%r.
- proof.
-  progress; fun; sp.
-  while  
-   (let pms = decrypt () OW_PCA.OW_PCA.sk pv c in
-    (forall x, mem x q => in_dom x B.m) /\
-    (forall x, 
-     in_dom x B.m => !mem x q => maybe_pms = None => pms <> fst (snd x)) /\
-    (maybe_pms <> None =>
-     (exists h t, in_dom (h, (pms, t)) B.m) /\ maybe_pms = Some pms))
-   (card q).
-   intros z; sp; wp. 
-   exists * pms, pv, c; elim *; intros pms pv c.
-   by call (check_spec () pms pv c); skip; progress; smt. 
-  by wp; skip; progress; smt.
- qed.
-
- local lemma find_spec : forall (_pv:version) (_c:ciphertext) (_h:hash) (_t:label),
-   bd_hoare 
-   [ B(OW_PCA.OW_PCA(PMS_KEM, B).O).find : 
-     pv = _pv /\ c = _c /\ h = _h /\ t = _t ==> 
-     let pms = decrypt () OW_PCA.OW_PCA.sk _pv _c in
-      (in_dom (_h, (pms, _t)) B.m <=> res = Some pms) /\
-      (res <> None => res = Some pms) ] = 1%r.
- proof.
-  progress; fun; sp.
-  while  
-   (let pms = decrypt () OW_PCA.OW_PCA.sk pv c in
-    (forall x, mem x q => in_dom x B.m) /\
-    (forall x, 
-     in_dom x B.m => !mem x q => maybe_pms = None => x <> (h, (pms, t))) /\
-    (maybe_pms <> None => 
-     in_dom (h, (pms, t)) B.m /\ maybe_pms = Some pms /\ h = h' /\  t = t'))
-   (card q).
-   intros z; sp; wp. 
-   exists * pms, pv, c; elim *; intros pms pv c.
-   by call (check_spec () pms pv c); skip; progress; smt. 
-  by wp; skip; progress; smt.
- qed.
-
- local equiv RCCA2_OW_extract : 
-   RCCA2.O.extract ~ B(OW_PCA.OW_PCA(PMS_KEM, B).O).O.extract :
-   ={p, s} /\ ={V.keys, V.labels, V.guess, V.t, V.c} /\
-   V.sk{1} = OW_PCA.OW_PCA.sk{2} /\ RCCA2.m{1} = B.m{2} /\ RCCA2.d{1} = B.d{2} 
-   ==>
-   ={res} /\ ={V.keys, V.labels, V.guess, V.t, V.c} /\
-   V.sk{1} = OW_PCA.OW_PCA.sk{2} /\ RCCA2.m{1} = B.m{2} /\ RCCA2.d{1} = B.d{2}. 
- proof.
-  fun.
-  sp; if => //.
-   seq 0 2 : 
-    (={pms, t, p, s, V.keys, V.labels, V.guess, V.t, V.c} /\
-     V.sk{1} = OW_PCA.OW_PCA.sk{2} /\ RCCA2.m{1} = B.m{2} /\ RCCA2.d{1} = B.d{2} /\
-     ((find_ext V.sk RCCA2.d p pms t){1} <=> 
-      (in_dom t B.d /\ p = h /\ found){2})).
-    sp; exists * pms{2}, pv{2}, c{2}; elim *; intros pms pv c.
-    by call{2} (check_spec () pms pv c); skip; progress; smt.
-    by if => //; wp; try rnd; skip; progress.
-   by wp.
- qed.
-
- local equiv RCCA2_OW_dec : 
-   RCCA2.O.dec ~ B(OW_PCA.OW_PCA(PMS_KEM, B).O).O.dec :
-   ={p, t, c} /\ ={V.keys, V.labels, V.guess, V.t, V.c} /\
-   V.sk{1} = OW_PCA.OW_PCA.sk{2} /\ RCCA2.m{1} = B.m{2} /\ RCCA2.d{1} = B.d{2} 
-   ==>
-   ={res} /\ ={V.keys, V.labels, V.guess, V.t, V.c} /\
-   V.sk{1} = OW_PCA.OW_PCA.sk{2} /\ RCCA2.m{1} = B.m{2} /\ RCCA2.d{1} = B.d{2}. 
- proof.
-  fun.
-  sp; if => //.
-  sp; if => //.
-  seq 0 1 :    
-   (maybe_k{1} = None /\
-    ={maybe_k, pv, h, p, t, c, V.labels, V.keys, V.guess, V.t, V.c} /\
-    V.sk{1} = OW_PCA.OW_PCA.sk{2} /\
-    RCCA2.m{1} = B.m{2} /\ RCCA2.d{1} = B.d{2} /\
-    !(V.guess /\ (pv, h) = p' /\ t = V.t /\ V.c = c){1} /\
-    ((find_dec V.sk RCCA2.m pv c h t){1} <=> maybe_pms{2} <> None) /\
-    (maybe_pms <> None => 
-     maybe_pms = Some (decrypt () OW_PCA.OW_PCA.sk pv c)){2}).
-   sp; exists * pv{2}, c{2}, h{2}, t{2}; elim *; intros pv c h t.
-   by call{2} (find_spec pv c h t); skip; progress; smt.
-
-   if => //.
-    by wp; skip; smt.
-    by wp; rnd.
- qed.
- 
- local equiv RCCA2_OW :
-  RCCA2.main ~ OW_PCA.OW_PCA(PMS_KEM, B).main :
-  true ==> (exists t, in_dom (snd p', (V.pms, t)) RCCA2.m){1} => res{2}.
- proof.
-  fun.
-  (* Workaround to swap PMS_KEM.enc *)
-  transitivity {1} {
-   PMS_KEM.init();
-   (pk, V.sk) = PMS_KEM.keygen();
-   V.init();
-   RCCA2.m = Core.empty;
-   RCCA2.d = Core.empty;
-   V.t = RCCA2.A.choose(pk);
-   (V.pms, V.c) = PMS_KEM.enc((), pk, fst p');
-   k0 = $Outer_KEM.key;
-   k1 = $Outer_KEM.key;
-   V.guess = true;
-   V.keys = add k0 (add k1 V.keys);
-   b' = RCCA2.A.guess(V.c, k0);
-  }
-  (true ==> ={glob V, RCCA2.m, RCCA2.d})
-  (true ==> (exists t, in_dom (snd p', (V.pms, t)) RCCA2.m){1} => (k = k'){2}) => //.
-  call (_: ={glob V, RCCA2.m, RCCA2.d}).
-   by fun; eqobs_in.
-   by fun; eqobs_in.
-   wp; rnd; rnd; simplify.
-   admit (* swap{1} 6 1, but technically dec 'uses' V.c *).
-  (*********************************)
-  inline OW_PCA.OW_PCA(PMS_KEM, B).A.choose OW_PCA.OW_PCA(PMS_KEM, B).A.guess.
-  wp; seq 6 7 : (={pk, glob A, V.keys, V.labels, V.guess, V.t, V.c} /\ 
-   V.sk{1} = OW_PCA.OW_PCA.sk{2} /\ 
-   RCCA2.m{1} = B.m{2} /\ RCCA2.d{1} = B.d{2}).
-   call (_: ={V.keys, V.labels, V.guess, V.t, V.c} /\
-    V.sk{1} = OW_PCA.OW_PCA.sk{2} /\ RCCA2.m{1} = B.m{2} /\ RCCA2.d{1} = B.d{2}).
-    by apply RCCA2_OW_dec.
-    by apply RCCA2_OW_extract.
-   by inline V.init; wp; call (_:true); wp; call (_:true).
-
-   seq 1 2 :
-    (={pk, glob A, V.keys, V.labels, V.guess, V.t} /\
-     (decrypt () V.sk (fst p') V.c = V.pms){1} /\
-     V.pms{1} = k{2} /\ V.c{1} = c{2} /\
-     V.sk{1} = OW_PCA.OW_PCA.sk{2} /\ 
-     RCCA2.m{1} = B.m{2} /\ RCCA2.d{1} = B.d{2}).
-   exists * V.sk{1}, pk{1}; elim *; intros sk pk.
-   by call (enc_spec_rel pk sk (fst p')); wp; skip; smt.
- 
-   seq 5 7 : (={pk, glob A, V.keys, V.labels, V.guess, V.t, V.c} /\ 
-    V.sk{1} = OW_PCA.OW_PCA.sk{2} /\ 
-    V.pms{1} = k{2} /\
-    (decrypt () V.sk (fst p') V.c = V.pms){1} /\
-    V.pms{1} = k{2} /\ V.c{1} = c0{2} /\
-    RCCA2.m{1} = B.m{2} /\ RCCA2.d{1} = B.d{2}).
+  local equiv RCCA2_NR :
+    RCCA2.main ~ PCA.NR_PCA(PMS_KEM, C).main :
+    true ==> 
+    (let (k, pv, h, c) = proj RCCA2.d.[V.t] in
+       c <> V.c /\ decrypt V.sk pv c = V.pms){1} => res{2}.
+  proof.
+   fun.
+   (* Workaround to swap PMS_KEM.enc *)
+   transitivity {1} {
+     PMS_KEM.init();
+     (pk, V.sk) = PMS_KEM.keygen();
+     V.init();
+     RCCA2.m = Core.empty;
+     RCCA2.d = Core.empty;
+     V.t = RCCA2.A.choose(pk);
+     (V.pms, V.c) = PMS_KEM.enc((), pk, fst pp);
+     k0 = $key;
+     k1 = $key;
+     V.guess = true;
+     V.keys = add k0 (add k1 V.keys);
+     b' = RCCA2.A.guess(V.c, k0);
+   }
+   (true ==> ={glob V, RCCA2.m, RCCA2.d})
+   (true ==> 
+    (let (k, pv, h, c) = proj RCCA2.d.[V.t] in
+     c <> V.c /\ decrypt V.sk pv c = V.pms){1} => (c <> c' /\ k' = k){2}) => //.
+   call (_: ={glob V, RCCA2.m, RCCA2.d}).
+     by fun; eqobs_in.
+     by fun; eqobs_in.
+    wp; rnd; rnd; simplify.
+    seq 5 5 : (={glob V, pk, RCCA2.m, RCCA2.d}); first by eqobs_in.
+    seq 2 2 : (={glob A, glob V, pk, RCCA2.m, RCCA2.d}).
+      admit (* swap, but technically dec 'uses' V.c *).
+      by skip.
+   (*********************************)
+   inline PCA.NR_PCA(PMS_KEM, C).A.choose 
+          PCA.NR_PCA(PMS_KEM, C).A.guess.
+   wp; seq 6 7 : (={pk, glob A, V.keys, V.labels, V.guess, V.t, V.c} /\
+    keypair(pk, V.sk){1} /\
+    V.sk{1} = PCA.V.sk{2} /\ 
+    RCCA2.m{1} = Find.m{2} /\ RCCA2.d{1} = Find.d{2}).
     call (_: ={V.keys, V.labels, V.guess, V.t, V.c} /\
-     V.sk{1} = OW_PCA.OW_PCA.sk{2} /\ RCCA2.m{1} = B.m{2} /\ RCCA2.d{1} = B.d{2}).
+     V.sk{1} = PCA.V.sk{2} /\ 
+     RCCA2.m{1} = Find.m{2} /\ RCCA2.d{1} = Find.d{2}).
      by apply RCCA2_OW_dec.
      by apply RCCA2_OW_extract.
-    by wp; rnd; rnd; wp; skip.
-
-   exists * c0{2}; elim *; intros c.
-   call{2} (find_any_spec (fst p') c).
-   by wp; skip; progress; smt.
- qed.
-
- local lemma Pr_RCCA2_OW : forall &m,
-   Pr[RCCA2.main() @ &m : exists t, in_dom (snd p', (V.pms, t)) RCCA2.m] <=
-   Pr[OW_PCA.OW_PCA(PMS_KEM, B).main() @ &m : res].
- proof.
-  by intros &m; equiv_deno RCCA2_OW.
- qed.
-
-
- (** RCCA2 -> NR *)
-
- local module C(PCO:NR_PCA.Oracles) = {
-  var m : (hash * (pms * label), ms) map
-  var d : (label, (ms * version * hash * ciphertext)) map
-
-  (* Private procedures *)
-  fun find(pv:version, c:ciphertext, h:hash, t:label) : pms option = {
-    var h' : hash;
-    var s : pms * label;
-    var pms : pms;
-    var t' : label;
-    var found : bool;
-    var q : (hash * (pms * label)) set;
-    var maybe_pms : pms option = None;
-    q = dom(m);
-    while (q <> FSet.empty /\ maybe_pms = None) {
-      (h',  s) = pick q;
-      q = rm (h', s) q;
-      (pms, t') = s;
-      found = PCO.check((), pms, pv, c);
-      maybe_pms = if found /\ h = h' /\ t = t' then Some pms else None; 
-    }
-    return maybe_pms;
-  }
-
-  fun find_any(pv:version, c:ciphertext) : pms option = {
-    var h' : hash;
-    var s : pms * label;
-    var pms : pms;
-    var t' : label;
-    var found : bool;
-    var q : (hash * (pms * label)) set;
-    var maybe_pms : pms option = None;
-    q = dom(m);
-    while (q <> FSet.empty /\ maybe_pms = None) {
-      (h',  s) = pick q;
-      q = rm (h', s) q;
-      (pms, t') = s;
-      found = PCO.check((), pms, pv, c);
-      maybe_pms = if found then Some pms else None; 
-    }
-    return maybe_pms;
-  }
-
-  module O = {
-   fun extract(p:hash, s:pms * label) : ms = {
-     var k : ms;
-     var pms : pms;
-     var t : label;
-     var pv : version;
-     var h : hash;
-     var c : ciphertext;
-     var found : bool;
-     (pms, t) = s;
-     if (!in_dom (p, (pms, t)) m) {
-       (k, pv, h, c) = proj d.[t];
-       found = PCO.check((), pms, pv, c);
-       if (in_dom t d /\ p = h /\ found) {
-         k = let (ms, pv, h, c) = proj d.[t] in ms;
-       }
-       else k = $Outer_KEM.key;
-       m.[(p, (pms, t))] = k;
-     }
-     else {
-       k = proj m.[(p, (pms, t))];
-     }
-     return k;
-   }
-
-   fun dec(p:version * hash, t:label, c:ciphertext) : ms option = {
-     var pv : version;
-     var h : hash;
-     var k : ms;
-     var maybe_pms : pms option;
-     var maybe_k : ms option = None;
-     if (!mem t V.labels /\ mem p P) { 
-       V.labels = add t V.labels;
-       (pv, h) = p;
-       if (!(V.guess /\ (pv, h) = p' /\ t = V.t /\ V.c = c)) {
-         maybe_pms = find(pv, c, h, t);
-         if (maybe_pms <> None) {
-           k = proj m.[(h, (proj maybe_pms, t))];
-         }
-         else {
-           k = $Outer_KEM.key;
-         }
-         d.[t] = (k, pv, h, c);
-         maybe_k = if (!mem k V.keys) then Some k else None;
-       }
-     }
-     return maybe_k;
-   }
-  }
+    by inline V.init; wp; call keygen_rel; wp; call (_:true); skip; smt.
   
-  module A = A(O, O)
+    seq 6 9 : (={b', pk, glob A, V.keys, V.labels, V.guess, V.t, V.c} /\
+     V.sk{1} = PCA.V.sk{2} /\ 
+     V.c{1} = c{2} /\ V.pms{1} = k{2} /\
+     (decrypt V.sk (fst pp) V.c = V.pms){1} /\
+     RCCA2.m{1} = Find.m{2} /\ RCCA2.d{1} = Find.d{2}). 
+    call (_: ={V.keys, V.labels, V.guess, V.t, V.c} /\
+     V.sk{1} = PCA.V.sk{2} /\ 
+     RCCA2.m{1} = Find.m{2} /\ 
+     RCCA2.d{1} = Find.d{2}).
+      by apply RCCA2_OW_dec.
+      by apply RCCA2_OW_extract.
   
-  fun choose(pk:pkey) : version = {
-    var t : label;
-    V.init();
-    m = Core.empty;
-    d = Core.empty;
-    V.t = A.choose(pk);
-    return (fst p');
-  }
-
-  fun guess(c:ciphertext) : version * ciphertext = {
-    var pms : pms;
-    var k0, k1 : ms;
-    var b' : bool;
-    V.c = c;
-    k0 = $Outer_KEM.key;
-    k1 = $Outer_KEM.key;
-    V.keys = add k0 (add k1 V.keys);
-    V.guess = true;
-    b' = A.guess(c, k0);
-    return let (k, pv, h, c) = proj d.[V.t] in (pv, c);
-  }
- }.
-
- local lemma check_spec' : forall _p _k _t _c,
-   bd_hoare 
-   [ NR_PCA.NR_PCA(PMS_KEM, C).O.check : 
-     p = _p /\ k = _k /\ t = _t /\ c = _c ==>
-    res <=> _k = decrypt _p NR_PCA.NR_PCA.sk _t _c ] = 1%r.
- proof.
-  progress; fun.
-  exists * NR_PCA.NR_PCA.sk; elim *; intros sk.
-  by call (dec_spec sk _t _c); skip; progress; smt.
- qed.
-
- local lemma find_any_spec' : forall (_pv:version) (_c:ciphertext),
-   bd_hoare 
-   [ C(NR_PCA.NR_PCA(PMS_KEM, C).O).find_any : 
-     pv = _pv /\ c = _c ==> 
-     let pms = decrypt () NR_PCA.NR_PCA.sk _pv _c in
-      ((exists h t, in_dom (h, (pms, t)) C.m) <=> res = Some pms) /\
-      (res <> None => res = Some pms)] = 1%r.
- proof.
-  progress; fun; sp.
-  while  
-   (let pms = decrypt () NR_PCA.NR_PCA.sk pv c in
-    (forall x, mem x q => in_dom x C.m) /\
-    (forall x, 
-     in_dom x C.m => !mem x q => maybe_pms = None => pms <> fst (snd x)) /\
-    (maybe_pms <> None =>
-     (exists h t, in_dom (h, (pms, t)) C.m) /\ maybe_pms = Some pms))
-   (card q).
-   intros z; sp; wp. 
-   exists * pms, pv, c; elim *; intros pms pv c.
-   by call (check_spec' () pms pv c); skip; progress; smt. 
-  by wp; skip; progress; smt.
- qed.
-
- local lemma find_spec' : forall (_pv:version) (_c:ciphertext) (_h:hash) (_t:label),
-   bd_hoare 
-   [ C(NR_PCA.NR_PCA(PMS_KEM, C).O).find : 
-     pv = _pv /\ c = _c /\ h = _h /\ t = _t ==> 
-     let pms = decrypt () NR_PCA.NR_PCA.sk _pv _c in
-      (in_dom (_h, (pms, _t)) C.m <=> res = Some pms) /\
-      (res <> None => res = Some pms) ] = 1%r.
- proof.
-  progress; fun; sp.
-  while  
-   (let pms = decrypt () NR_PCA.NR_PCA.sk pv c in
-    (forall x, mem x q => in_dom x C.m) /\
-    (forall x, 
-     in_dom x C.m => !mem x q => maybe_pms = None => x <> (h, (pms, t))) /\
-    (maybe_pms <> None => 
-     in_dom (h, (pms, t)) C.m /\ maybe_pms = Some pms /\ h = h' /\  t = t'))
-   (card q).
-   intros z; sp; wp. 
-   exists * pms, pv, c; elim *; intros pms pv c.
-   by call (check_spec' () pms pv c); skip; progress; smt. 
-  by wp; skip; progress; smt.
- qed.
-
- local equiv RCCA2_NR_extract : 
-   RCCA2.O.extract ~ C(NR_PCA.NR_PCA(PMS_KEM, C).O).O.extract :
-   ={p, s} /\ ={V.keys, V.labels, V.guess, V.t, V.c} /\
-   V.sk{1} = NR_PCA.NR_PCA.sk{2} /\ RCCA2.m{1} = C.m{2} /\ RCCA2.d{1} = C.d{2} 
-   ==>
-   ={res} /\ ={V.keys, V.labels, V.guess, V.t, V.c} /\
-   V.sk{1} = NR_PCA.NR_PCA.sk{2} /\ RCCA2.m{1} = C.m{2} /\ RCCA2.d{1} = C.d{2}. 
- proof.
-  fun.
-  sp; if => //.
-   seq 0 2 : 
-    (={pms, t, p, s, V.keys, V.labels, V.guess, V.t, V.c} /\
-     V.sk{1} = NR_PCA.NR_PCA.sk{2} /\ RCCA2.m{1} = C.m{2} /\ RCCA2.d{1} = C.d{2} /\
-     ((find_ext V.sk RCCA2.d p pms t){1} <=> 
-      (in_dom t C.d /\ p = h /\ found){2})).
-    sp; exists * pms{2}, pv{2}, c{2}; elim *; intros pms pv c.
-    by call{2} (check_spec' () pms pv c); skip; progress; smt.
-    by if => //; wp; try rnd; skip; progress.
-   by wp.
- qed.
-
- local equiv RCCA2_NR_dec : 
-   RCCA2.O.dec ~ C(NR_PCA.NR_PCA(PMS_KEM, C).O).O.dec :
-   ={p, t, c} /\ ={V.keys, V.labels, V.guess, V.t, V.c} /\
-   V.sk{1} = NR_PCA.NR_PCA.sk{2} /\ RCCA2.m{1} = C.m{2} /\ RCCA2.d{1} = C.d{2} 
-   ==>
-   ={res} /\ ={V.keys, V.labels, V.guess, V.t, V.c} /\
-   V.sk{1} = NR_PCA.NR_PCA.sk{2} /\ RCCA2.m{1} = C.m{2} /\ RCCA2.d{1} = C.d{2}. 
- proof.
-  fun.
-  sp; if => //.
-  sp; if => //.
-  seq 0 1 :    
-   (maybe_k{1} = None /\
-    ={maybe_k, pv, h, p, t, c, V.labels, V.keys, V.guess, V.t, V.c} /\
-    V.sk{1} = NR_PCA.NR_PCA.sk{2} /\
-    RCCA2.m{1} = C.m{2} /\ RCCA2.d{1} = C.d{2} /\
-    !(V.guess /\ (pv, h) = p' /\ t = V.t /\ V.c = c){1} /\
-    ((find_dec V.sk RCCA2.m pv c h t){1} <=> maybe_pms{2} <> None) /\
-    (maybe_pms <> None => 
-     maybe_pms = Some (decrypt () NR_PCA.NR_PCA.sk pv c)){2}).
-   sp; exists * pv{2}, c{2}, h{2}, t{2}; elim *; intros pv c h t.
-   by call{2} (find_spec' pv c h t); skip; progress; smt.
-
-   if => //.
-    by wp; skip; smt.
-    by wp; rnd.
- qed.
- 
- local equiv RCCA2_NR :
-  RCCA2.main ~ NR_PCA.NR_PCA(PMS_KEM, C).main :
-  true ==> 
-  (let (k, pv, h, c) = proj RCCA2.d.[V.t] in
-    c <> V.c /\ decrypt () V.sk pv c = V.pms){1} => res{2}.
- proof.
-  fun.
-  (* Workaround to swap PMS_KEM.enc *)
-  transitivity {1} {
-   PMS_KEM.init();
-   (pk, V.sk) = PMS_KEM.keygen();
-   V.init();
-   RCCA2.m = Core.empty;
-   RCCA2.d = Core.empty;
-   V.t = RCCA2.A.choose(pk);
-   (V.pms, V.c) = PMS_KEM.enc((), pk, fst p');
-   k0 = $Outer_KEM.key;
-   k1 = $Outer_KEM.key;
-   V.guess = true;
-   V.keys = add k0 (add k1 V.keys);
-   b' = RCCA2.A.guess(V.c, k0);
-  }
-  (true ==> ={glob V, RCCA2.m, RCCA2.d})
-  (true ==> 
-   (let (k, pv, h, c) = proj RCCA2.d.[V.t] in
-    c <> V.c /\ decrypt () V.sk pv c = V.pms){1} => (c <> c' /\ k' = k){2}) => //.
-  call (_: ={glob V, RCCA2.m, RCCA2.d}).
-   by fun; eqobs_in.
-   by fun; eqobs_in.
-   wp; rnd; rnd; simplify.
-   admit (* swap{1} 6 1, but technically dec 'uses' V.c *).
-  (*********************************)
-  inline NR_PCA.NR_PCA(PMS_KEM, C).A.choose NR_PCA.NR_PCA(PMS_KEM, C).A.guess.
-  wp; seq 6 7 : (={pk, glob A, V.keys, V.labels, V.guess, V.t, V.c} /\ 
-   V.sk{1} = NR_PCA.NR_PCA.sk{2} /\ 
-   RCCA2.m{1} = C.m{2} /\ RCCA2.d{1} = C.d{2}).
-   call (_: ={V.keys, V.labels, V.guess, V.t, V.c} /\
-    V.sk{1} = NR_PCA.NR_PCA.sk{2} /\ RCCA2.m{1} = C.m{2} /\ RCCA2.d{1} = C.d{2}).
-    by apply RCCA2_NR_dec.
-    by apply RCCA2_NR_extract.
-   inline V.init; wp; call (_:true); wp; call (_:true); skip; progress.
-
-   seq 6 9 : (={b', pk, glob A, V.keys, V.labels, V.guess, V.t, V.c} /\
-    V.sk{1} = NR_PCA.NR_PCA.sk{2} /\ 
-    V.c{1} = c{2} /\ V.pms{1} = k{2} /\
-    (decrypt () V.sk (fst p') V.c = V.pms){1} /\
-    RCCA2.m{1} = C.m{2} /\ RCCA2.d{1} = C.d{2}). 
-   call (_: ={V.keys, V.labels, V.guess, V.t, V.c} /\
-    V.sk{1} = NR_PCA.NR_PCA.sk{2} /\ RCCA2.m{1} = C.m{2} /\ RCCA2.d{1} = C.d{2}).
-    by apply RCCA2_NR_dec.
-    by apply RCCA2_NR_extract.
-
-   wp; rnd; rnd; wp.
-   exists * V.sk{1}, pk{1}; elim *; intros sk pk.
-   call (enc_spec_rel pk sk (fst p')).
-   wp; skip; progress; smt.
-
-   sp; wp; exists * NR_PCA.NR_PCA.sk{2}, t'{2}, c'{2}; elim *; intros sk pv c.
-   call{2} (dec_spec sk pv c).
-   by skip; progress; smt.
- qed.
-
- local lemma Pr_RCCA2_NR : forall &m,
-   Pr[RCCA2.main() @ &m : let (k, pv, h, c) = proj RCCA2.d.[V.t] in
-      c <> V.c /\ decrypt () V.sk pv c = V.pms] <=
-   Pr[NR_PCA.NR_PCA(PMS_KEM, C).main() @ &m : res].
- proof.
-  by intros &m; equiv_deno RCCA2_NR.
- qed.
-
- (** Conclusion **)
- lemma Conclusion : forall &m,
-   exists (B <: OW_PCA.Adversary {OW_PCA.OW_PCA}) 
-          (C <: NR_PCA.Adversary {NR_PCA.NR_PCA}),
-    Pr[RCCA(KEM(RO_KEF, PMS_KEM), A(RO_KEF)).main() @ &m : res] - 1%r / 2%r <=
-    Pr[OW_PCA.OW_PCA(PMS_KEM, B).main() @ &m : res] +
-    Pr[NR_PCA.NR_PCA(PMS_KEM, C).main() @ &m : res].
- proof.
-  intros &m; exists B, C.
-  cut X : forall (x y z:real), 0%r <= z => x <= y + z => x - y <= z by smt.
-  apply X; first by smt.
-  apply (Trans _ (1%r / 2%r + Pr[RCCA1.main() @ &m : RCCA1.abort])).
-   by apply (Pr_RCCA_RCCA1 &m).
-   apply addleM => //.
-   apply (Trans _
-    (Pr[RCCA2.main() @ &m : exists t, in_dom (snd p', (V.pms, t)) RCCA2.m] +  
-     Pr[RCCA2.main() @ &m : let (k, pv, h, c) = proj RCCA2.d.[V.t] in
-       c <> V.c /\ decrypt () V.sk pv c = V.pms])).
+    wp; rnd; rnd; wp.
+    exists * V.sk{1}, pk{1}; elim *; intros sk pk.
+    call (enc_spec_rel pk sk (fst pp)).
+    wp; skip; progress; smt.
+  
+    sp; wp; exists * PCA.V.sk{2}, t'{2}, c'{2}; elim *; intros sk pv c.
+    call{2} (dec_spec sk pv c).
+    by skip; progress; smt.
+  qed.
+  
+  local lemma Pr_RCCA2_NR : forall &m,
+    Pr[RCCA2.main() @ &m : let (k, pv, h, c) = proj RCCA2.d.[V.t] in
+       c <> V.c /\ decrypt V.sk pv c = V.pms] <=
+    Pr[PCA.NR_PCA(PMS_KEM, C).main() @ &m : res].
+  proof.
+    by intros &m; equiv_deno RCCA2_NR.
+  qed.
+  
+  (** Conclusion **)
+  lemma Conclusion : forall &m,
+    exists (B <: PCA.OW_Adversary {PCA.V}) 
+           (C <: PCA.NR_Adversary {PCA.V}),
+     Pr[RCCA(KEM(RO_KEF, PMS_KEM), A(RO_KEF)).main() @ &m : res] - 1%r / 2%r <=
+     Pr[PCA.OW_PCA(PMS_KEM, B).main() @ &m : res] +
+     Pr[PCA.NR_PCA(PMS_KEM, C).main() @ &m : res].
+  proof.
+    intros &m; exists B, C.
+    cut X : forall (x y z), 0%r <= z => x <= y + z => x - y <= z by smt.
+    apply X; first by smt.
+    apply (Trans _ (1%r / 2%r + Pr[RCCA1.main() @ &m : RCCA1.abort]));
+    first by apply (Pr_RCCA_RCCA1 &m).
+    apply addleM => //.
+    apply (Trans _
+      (Pr[RCCA2.main() @ &m : exists t, in_dom (snd pp, (V.pms, t)) RCCA2.m] +  
+       Pr[RCCA2.main() @ &m : let (k, pv, h, c) = proj RCCA2.d.[V.t] in
+          c <> V.c /\ decrypt V.sk pv c = V.pms])).
     by apply (Pr_RCCA1_RCCA2 &m).
     apply addleM.
-     by apply (Pr_RCCA2_OW &m).
-     by apply (Pr_RCCA2_NR &m).
- qed.
+      by apply (Pr_RCCA2_OW &m).
+      by apply (Pr_RCCA2_NR &m).
+  qed.
 
 end section.
+
+print axiom Conclusion.
